<?xml version="1.0"?>
<rdf:RDF xmlns="http://www.semanticweb.org/cassandwich/ontologies/2018/2/podcast-ontology#"
     xml:base="http://www.semanticweb.org/cassandwich/ontologies/2018/2/podcast-ontology"
     xmlns:rdf="http://www.w3.org/1999/02/22-rdf-syntax-ns#"
     xmlns:owl="http://www.w3.org/2002/07/owl#"
     xmlns:xml="http://www.w3.org/XML/1998/namespace"
     xmlns:xsd="http://www.w3.org/2001/XMLSchema#"
     xmlns:rdfs="http://www.w3.org/2000/01/rdf-schema#">
    <owl:Ontology rdf:about="http://www.semanticweb.org/cassandwich/ontologies/2018/2/podcast-ontology">
        <rdfs:comment>A podcast ontology that describes various podcasts based on their properties.</rdfs:comment>
    </owl:Ontology>
    


    <!-- 
    ///////////////////////////////////////////////////////////////////////////////////////
    //
    // Object Properties
    //
    ///////////////////////////////////////////////////////////////////////////////////////
     -->

    


    <!-- http://www.semanticweb.org/cassandwich/ontologies/2018/2/podcast-ontology#has_number_of_hosts -->

    <owl:ObjectProperty rdf:about="http://www.semanticweb.org/cassandwich/ontologies/2018/2/podcast-ontology#has_number_of_hosts"/>
    


    <!-- http://www.semanticweb.org/cassandwich/ontologies/2018/2/podcast-ontology#is_categorized_as -->

    <owl:ObjectProperty rdf:about="http://www.semanticweb.org/cassandwich/ontologies/2018/2/podcast-ontology#is_categorized_as"/>
    


    <!-- http://www.semanticweb.org/cassandwich/ontologies/2018/2/podcast-ontology#is_from_country -->

    <owl:ObjectProperty rdf:about="http://www.semanticweb.org/cassandwich/ontologies/2018/2/podcast-ontology#is_from_country"/>
    


    <!-- http://www.semanticweb.org/cassandwich/ontologies/2018/2/podcast-ontology#is_genre -->

    <owl:ObjectProperty rdf:about="http://www.semanticweb.org/cassandwich/ontologies/2018/2/podcast-ontology#is_genre"/>
    


    <!-- 
    ///////////////////////////////////////////////////////////////////////////////////////
    //
    // Classes
    //
    ///////////////////////////////////////////////////////////////////////////////////////
     -->

    


    <!-- http://www.semanticweb.org/cassandwich/ontologies/2018/2/podcast-ontology#AKillingOnTheCape -->

    <owl:Class rdf:about="http://www.semanticweb.org/cassandwich/ontologies/2018/2/podcast-ontology#AKillingOnTheCape">
        <rdfs:subClassOf rdf:resource="http://www.semanticweb.org/cassandwich/ontologies/2018/2/podcast-ontology#PodcastTitle"/>
        <rdfs:subClassOf>
            <owl:Restriction>
                <owl:onProperty rdf:resource="http://www.semanticweb.org/cassandwich/ontologies/2018/2/podcast-ontology#has_number_of_hosts"/>
                <owl:someValuesFrom rdf:resource="http://www.semanticweb.org/cassandwich/ontologies/2018/2/podcast-ontology#One"/>
            </owl:Restriction>
        </rdfs:subClassOf>
        <rdfs:subClassOf>
            <owl:Restriction>
                <owl:onProperty rdf:resource="http://www.semanticweb.org/cassandwich/ontologies/2018/2/podcast-ontology#is_genre"/>
                <owl:someValuesFrom rdf:resource="http://www.semanticweb.org/cassandwich/ontologies/2018/2/podcast-ontology#NonFiction"/>
            </owl:Restriction>
        </rdfs:subClassOf>
        <rdfs:subClassOf>
            <owl:Restriction>
                <owl:onProperty rdf:resource="http://www.semanticweb.org/cassandwich/ontologies/2018/2/podcast-ontology#is_categorized_as"/>
                <owl:allValuesFrom rdf:resource="http://www.semanticweb.org/cassandwich/ontologies/2018/2/podcast-ontology#News&amp;Politics"/>
            </owl:Restriction>
        </rdfs:subClassOf>
        <rdfs:subClassOf>
            <owl:Restriction>
                <owl:onProperty rdf:resource="http://www.semanticweb.org/cassandwich/ontologies/2018/2/podcast-ontology#is_from_country"/>
                <owl:allValuesFrom rdf:resource="http://www.semanticweb.org/cassandwich/ontologies/2018/2/podcast-ontology#UnitedStates"/>
            </owl:Restriction>
        </rdfs:subClassOf>
        <rdfs:comment>Podcast is titled &apos;A Killing on the Cape&apos;.

Reference: https://itunes.apple.com/ca/podcast/a-killing-on-the-cape/id1298055025?mt=2</rdfs:comment>
    </owl:Class>
    


    <!-- http://www.semanticweb.org/cassandwich/ontologies/2018/2/podcast-ontology#Accused -->

    <owl:Class rdf:about="http://www.semanticweb.org/cassandwich/ontologies/2018/2/podcast-ontology#Accused">
        <rdfs:subClassOf rdf:resource="http://www.semanticweb.org/cassandwich/ontologies/2018/2/podcast-ontology#PodcastTitle"/>
        <rdfs:subClassOf>
            <owl:Restriction>
                <owl:onProperty rdf:resource="http://www.semanticweb.org/cassandwich/ontologies/2018/2/podcast-ontology#has_number_of_hosts"/>
                <owl:someValuesFrom rdf:resource="http://www.semanticweb.org/cassandwich/ontologies/2018/2/podcast-ontology#One"/>
            </owl:Restriction>
        </rdfs:subClassOf>
        <rdfs:subClassOf>
            <owl:Restriction>
                <owl:onProperty rdf:resource="http://www.semanticweb.org/cassandwich/ontologies/2018/2/podcast-ontology#is_genre"/>
                <owl:someValuesFrom rdf:resource="http://www.semanticweb.org/cassandwich/ontologies/2018/2/podcast-ontology#NonFiction"/>
            </owl:Restriction>
        </rdfs:subClassOf>
        <rdfs:subClassOf>
            <owl:Restriction>
                <owl:onProperty rdf:resource="http://www.semanticweb.org/cassandwich/ontologies/2018/2/podcast-ontology#is_categorized_as"/>
                <owl:allValuesFrom rdf:resource="http://www.semanticweb.org/cassandwich/ontologies/2018/2/podcast-ontology#News&amp;Politics"/>
            </owl:Restriction>
        </rdfs:subClassOf>
        <rdfs:subClassOf>
            <owl:Restriction>
                <owl:onProperty rdf:resource="http://www.semanticweb.org/cassandwich/ontologies/2018/2/podcast-ontology#is_from_country"/>
                <owl:allValuesFrom rdf:resource="http://www.semanticweb.org/cassandwich/ontologies/2018/2/podcast-ontology#UnitedStates"/>
            </owl:Restriction>
        </rdfs:subClassOf>
        <rdfs:comment>Podcast is titled &apos;Accused&apos;.

Reference: https://itunes.apple.com/ca/podcast/accused/id1145990861?mt=2</rdfs:comment>
    </owl:Class>
    


    <!-- http://www.semanticweb.org/cassandwich/ontologies/2018/2/podcast-ontology#AliceIsntDead -->

    <owl:Class rdf:about="http://www.semanticweb.org/cassandwich/ontologies/2018/2/podcast-ontology#AliceIsntDead">
        <rdfs:subClassOf rdf:resource="http://www.semanticweb.org/cassandwich/ontologies/2018/2/podcast-ontology#PodcastTitle"/>
        <rdfs:subClassOf>
            <owl:Restriction>
                <owl:onProperty rdf:resource="http://www.semanticweb.org/cassandwich/ontologies/2018/2/podcast-ontology#has_number_of_hosts"/>
                <owl:someValuesFrom rdf:resource="http://www.semanticweb.org/cassandwich/ontologies/2018/2/podcast-ontology#Six"/>
            </owl:Restriction>
        </rdfs:subClassOf>
        <rdfs:subClassOf>
            <owl:Restriction>
                <owl:onProperty rdf:resource="http://www.semanticweb.org/cassandwich/ontologies/2018/2/podcast-ontology#is_categorized_as"/>
                <owl:allValuesFrom rdf:resource="http://www.semanticweb.org/cassandwich/ontologies/2018/2/podcast-ontology#PerformingArts"/>
            </owl:Restriction>
        </rdfs:subClassOf>
        <rdfs:subClassOf>
            <owl:Restriction>
                <owl:onProperty rdf:resource="http://www.semanticweb.org/cassandwich/ontologies/2018/2/podcast-ontology#is_from_country"/>
                <owl:allValuesFrom rdf:resource="http://www.semanticweb.org/cassandwich/ontologies/2018/2/podcast-ontology#UnitedStates"/>
            </owl:Restriction>
        </rdfs:subClassOf>
        <rdfs:subClassOf>
            <owl:Restriction>
                <owl:onProperty rdf:resource="http://www.semanticweb.org/cassandwich/ontologies/2018/2/podcast-ontology#is_genre"/>
                <owl:allValuesFrom rdf:resource="http://www.semanticweb.org/cassandwich/ontologies/2018/2/podcast-ontology#Fiction"/>
            </owl:Restriction>
        </rdfs:subClassOf>
        <rdfs:comment>Podcast is titled &apos;Alice Isn&apos;t Dead&apos;.

Reference: https://itunes.apple.com/ca/podcast/alice-isnt-dead/id1088978354?mt=2</rdfs:comment>
    </owl:Class>
    


    <!-- http://www.semanticweb.org/cassandwich/ontologies/2018/2/podcast-ontology#AloneALoveStory -->

    <owl:Class rdf:about="http://www.semanticweb.org/cassandwich/ontologies/2018/2/podcast-ontology#AloneALoveStory">
        <rdfs:subClassOf rdf:resource="http://www.semanticweb.org/cassandwich/ontologies/2018/2/podcast-ontology#PodcastTitle"/>
        <rdfs:subClassOf>
            <owl:Restriction>
                <owl:onProperty rdf:resource="http://www.semanticweb.org/cassandwich/ontologies/2018/2/podcast-ontology#has_number_of_hosts"/>
                <owl:allValuesFrom rdf:resource="http://www.semanticweb.org/cassandwich/ontologies/2018/2/podcast-ontology#One"/>
            </owl:Restriction>
        </rdfs:subClassOf>
        <rdfs:subClassOf>
            <owl:Restriction>
                <owl:onProperty rdf:resource="http://www.semanticweb.org/cassandwich/ontologies/2018/2/podcast-ontology#is_categorized_as"/>
                <owl:allValuesFrom rdf:resource="http://www.semanticweb.org/cassandwich/ontologies/2018/2/podcast-ontology#Society&amp;Culture"/>
            </owl:Restriction>
        </rdfs:subClassOf>
        <rdfs:subClassOf>
            <owl:Restriction>
                <owl:onProperty rdf:resource="http://www.semanticweb.org/cassandwich/ontologies/2018/2/podcast-ontology#is_from_country"/>
                <owl:allValuesFrom rdf:resource="http://www.semanticweb.org/cassandwich/ontologies/2018/2/podcast-ontology#Canada"/>
            </owl:Restriction>
        </rdfs:subClassOf>
        <rdfs:subClassOf>
            <owl:Restriction>
                <owl:onProperty rdf:resource="http://www.semanticweb.org/cassandwich/ontologies/2018/2/podcast-ontology#is_genre"/>
                <owl:allValuesFrom rdf:resource="http://www.semanticweb.org/cassandwich/ontologies/2018/2/podcast-ontology#NonFiction"/>
            </owl:Restriction>
        </rdfs:subClassOf>
        <rdfs:comment>Podcast is titled &apos;Alone: A Love Story&apos;.

Reference: https://itunes.apple.com/ca/podcast/alone-a-love-story/id1276619662?mt=2</rdfs:comment>
    </owl:Class>
    


    <!-- http://www.semanticweb.org/cassandwich/ontologies/2018/2/podcast-ontology#Ambushed -->

    <owl:Class rdf:about="http://www.semanticweb.org/cassandwich/ontologies/2018/2/podcast-ontology#Ambushed">
        <rdfs:subClassOf rdf:resource="http://www.semanticweb.org/cassandwich/ontologies/2018/2/podcast-ontology#PodcastTitle"/>
        <rdfs:subClassOf>
            <owl:Restriction>
                <owl:onProperty rdf:resource="http://www.semanticweb.org/cassandwich/ontologies/2018/2/podcast-ontology#has_number_of_hosts"/>
                <owl:someValuesFrom rdf:resource="http://www.semanticweb.org/cassandwich/ontologies/2018/2/podcast-ontology#One"/>
            </owl:Restriction>
        </rdfs:subClassOf>
        <rdfs:subClassOf>
            <owl:Restriction>
                <owl:onProperty rdf:resource="http://www.semanticweb.org/cassandwich/ontologies/2018/2/podcast-ontology#is_categorized_as"/>
                <owl:allValuesFrom rdf:resource="http://www.semanticweb.org/cassandwich/ontologies/2018/2/podcast-ontology#News&amp;Politics"/>
            </owl:Restriction>
        </rdfs:subClassOf>
        <rdfs:subClassOf>
            <owl:Restriction>
                <owl:onProperty rdf:resource="http://www.semanticweb.org/cassandwich/ontologies/2018/2/podcast-ontology#is_from_country"/>
                <owl:allValuesFrom rdf:resource="http://www.semanticweb.org/cassandwich/ontologies/2018/2/podcast-ontology#Canada"/>
            </owl:Restriction>
        </rdfs:subClassOf>
        <rdfs:subClassOf>
            <owl:Restriction>
                <owl:onProperty rdf:resource="http://www.semanticweb.org/cassandwich/ontologies/2018/2/podcast-ontology#is_genre"/>
                <owl:allValuesFrom rdf:resource="http://www.semanticweb.org/cassandwich/ontologies/2018/2/podcast-ontology#NonFiction"/>
            </owl:Restriction>
        </rdfs:subClassOf>
        <rdfs:comment>Podcast is titled &apos;Ambushed&apos;.

Reference: https://itunes.apple.com/ca/podcast/ambushed/id1325243884?mt=2</rdfs:comment>
    </owl:Class>
    


    <!-- http://www.semanticweb.org/cassandwich/ontologies/2018/2/podcast-ontology#AnotherRound -->

    <owl:Class rdf:about="http://www.semanticweb.org/cassandwich/ontologies/2018/2/podcast-ontology#AnotherRound">
        <rdfs:subClassOf rdf:resource="http://www.semanticweb.org/cassandwich/ontologies/2018/2/podcast-ontology#PodcastTitle"/>
        <rdfs:subClassOf>
            <owl:Restriction>
                <owl:onProperty rdf:resource="http://www.semanticweb.org/cassandwich/ontologies/2018/2/podcast-ontology#has_number_of_hosts"/>
                <owl:someValuesFrom rdf:resource="http://www.semanticweb.org/cassandwich/ontologies/2018/2/podcast-ontology#Two"/>
            </owl:Restriction>
        </rdfs:subClassOf>
        <rdfs:subClassOf>
            <owl:Restriction>
                <owl:onProperty rdf:resource="http://www.semanticweb.org/cassandwich/ontologies/2018/2/podcast-ontology#is_categorized_as"/>
                <owl:someValuesFrom rdf:resource="http://www.semanticweb.org/cassandwich/ontologies/2018/2/podcast-ontology#Philosophy"/>
            </owl:Restriction>
        </rdfs:subClassOf>
        <rdfs:subClassOf>
            <owl:Restriction>
                <owl:onProperty rdf:resource="http://www.semanticweb.org/cassandwich/ontologies/2018/2/podcast-ontology#is_genre"/>
                <owl:someValuesFrom rdf:resource="http://www.semanticweb.org/cassandwich/ontologies/2018/2/podcast-ontology#NonFiction"/>
            </owl:Restriction>
        </rdfs:subClassOf>
        <rdfs:subClassOf>
            <owl:Restriction>
                <owl:onProperty rdf:resource="http://www.semanticweb.org/cassandwich/ontologies/2018/2/podcast-ontology#is_from_country"/>
                <owl:allValuesFrom rdf:resource="http://www.semanticweb.org/cassandwich/ontologies/2018/2/podcast-ontology#UnitedStates"/>
            </owl:Restriction>
        </rdfs:subClassOf>
        <rdfs:comment>Podcast is titled &apos;Another Round&apos;.

Reference: https://itunes.apple.com/ca/podcast/another-round/id977676980?mt=2</rdfs:comment>
    </owl:Class>
    


    <!-- http://www.semanticweb.org/cassandwich/ontologies/2018/2/podcast-ontology#Arts -->

    <owl:Class rdf:about="http://www.semanticweb.org/cassandwich/ontologies/2018/2/podcast-ontology#Arts">
        <rdfs:subClassOf rdf:resource="http://www.semanticweb.org/cassandwich/ontologies/2018/2/podcast-ontology#PodcastCategory"/>
        <rdfs:comment>The category defined by iTunes as Arts.

Reference: https://itunes.apple.com/ca/genre/podcasts-arts/id1301?mt=2</rdfs:comment>
    </owl:Class>
    


    <!-- http://www.semanticweb.org/cassandwich/ontologies/2018/2/podcast-ontology#AtlantaMonster -->

    <owl:Class rdf:about="http://www.semanticweb.org/cassandwich/ontologies/2018/2/podcast-ontology#AtlantaMonster">
        <rdfs:subClassOf rdf:resource="http://www.semanticweb.org/cassandwich/ontologies/2018/2/podcast-ontology#PodcastTitle"/>
        <rdfs:subClassOf>
            <owl:Restriction>
                <owl:onProperty rdf:resource="http://www.semanticweb.org/cassandwich/ontologies/2018/2/podcast-ontology#has_number_of_hosts"/>
                <owl:allValuesFrom rdf:resource="http://www.semanticweb.org/cassandwich/ontologies/2018/2/podcast-ontology#One"/>
            </owl:Restriction>
        </rdfs:subClassOf>
        <rdfs:subClassOf>
            <owl:Restriction>
                <owl:onProperty rdf:resource="http://www.semanticweb.org/cassandwich/ontologies/2018/2/podcast-ontology#is_categorized_as"/>
                <owl:allValuesFrom rdf:resource="http://www.semanticweb.org/cassandwich/ontologies/2018/2/podcast-ontology#Society&amp;Culture"/>
            </owl:Restriction>
        </rdfs:subClassOf>
        <rdfs:subClassOf>
            <owl:Restriction>
                <owl:onProperty rdf:resource="http://www.semanticweb.org/cassandwich/ontologies/2018/2/podcast-ontology#is_from_country"/>
                <owl:allValuesFrom rdf:resource="http://www.semanticweb.org/cassandwich/ontologies/2018/2/podcast-ontology#UnitedStates"/>
            </owl:Restriction>
        </rdfs:subClassOf>
        <rdfs:subClassOf>
            <owl:Restriction>
                <owl:onProperty rdf:resource="http://www.semanticweb.org/cassandwich/ontologies/2018/2/podcast-ontology#is_genre"/>
                <owl:allValuesFrom rdf:resource="http://www.semanticweb.org/cassandwich/ontologies/2018/2/podcast-ontology#NonFiction"/>
            </owl:Restriction>
        </rdfs:subClassOf>
        <rdfs:comment>Podcast is titled &apos;Atlanta Monster&apos;.

Reference: https://itunes.apple.com/ca/podcast/atlanta-monster/id1324249769?mt=2</rdfs:comment>
    </owl:Class>
    


    <!-- http://www.semanticweb.org/cassandwich/ontologies/2018/2/podcast-ontology#Australia -->

    <owl:Class rdf:about="http://www.semanticweb.org/cassandwich/ontologies/2018/2/podcast-ontology#Australia">
        <rdfs:subClassOf rdf:resource="http://www.semanticweb.org/cassandwich/ontologies/2018/2/podcast-ontology#PodcastCountryOfOrigin"/>
        <rdfs:comment>Country of origin is Australia.</rdfs:comment>
    </owl:Class>
    


    <!-- http://www.semanticweb.org/cassandwich/ontologies/2018/2/podcast-ontology#BlackHands -->

    <owl:Class rdf:about="http://www.semanticweb.org/cassandwich/ontologies/2018/2/podcast-ontology#BlackHands">
        <rdfs:subClassOf rdf:resource="http://www.semanticweb.org/cassandwich/ontologies/2018/2/podcast-ontology#PodcastTitle"/>
        <rdfs:subClassOf>
            <owl:Restriction>
                <owl:onProperty rdf:resource="http://www.semanticweb.org/cassandwich/ontologies/2018/2/podcast-ontology#has_number_of_hosts"/>
                <owl:someValuesFrom rdf:resource="http://www.semanticweb.org/cassandwich/ontologies/2018/2/podcast-ontology#One"/>
            </owl:Restriction>
        </rdfs:subClassOf>
        <rdfs:subClassOf>
            <owl:Restriction>
                <owl:onProperty rdf:resource="http://www.semanticweb.org/cassandwich/ontologies/2018/2/podcast-ontology#is_categorized_as"/>
                <owl:allValuesFrom rdf:resource="http://www.semanticweb.org/cassandwich/ontologies/2018/2/podcast-ontology#News&amp;Politics"/>
            </owl:Restriction>
        </rdfs:subClassOf>
        <rdfs:subClassOf>
            <owl:Restriction>
                <owl:onProperty rdf:resource="http://www.semanticweb.org/cassandwich/ontologies/2018/2/podcast-ontology#is_from_country"/>
                <owl:allValuesFrom rdf:resource="http://www.semanticweb.org/cassandwich/ontologies/2018/2/podcast-ontology#NewZealand"/>
            </owl:Restriction>
        </rdfs:subClassOf>
        <rdfs:subClassOf>
            <owl:Restriction>
                <owl:onProperty rdf:resource="http://www.semanticweb.org/cassandwich/ontologies/2018/2/podcast-ontology#is_genre"/>
                <owl:allValuesFrom rdf:resource="http://www.semanticweb.org/cassandwich/ontologies/2018/2/podcast-ontology#NonFiction"/>
            </owl:Restriction>
        </rdfs:subClassOf>
        <rdfs:comment>Podcast is titled &apos;Black Hands&apos;.

Reference: https://itunes.apple.com/ca/podcast/black-hands-a-family-mass-murder/id1259053911?mt=2</rdfs:comment>
    </owl:Class>
    


    <!-- http://www.semanticweb.org/cassandwich/ontologies/2018/2/podcast-ontology#Business -->

    <owl:Class rdf:about="http://www.semanticweb.org/cassandwich/ontologies/2018/2/podcast-ontology#Business">
        <rdfs:subClassOf rdf:resource="http://www.semanticweb.org/cassandwich/ontologies/2018/2/podcast-ontology#PodcastCategory"/>
        <rdfs:comment>The category defined by iTunes as Business.

Reference: https://itunes.apple.com/ca/genre/podcasts-business/id1321?mt=2</rdfs:comment>
    </owl:Class>
    


    <!-- http://www.semanticweb.org/cassandwich/ontologies/2018/2/podcast-ontology#Canada -->

    <owl:Class rdf:about="http://www.semanticweb.org/cassandwich/ontologies/2018/2/podcast-ontology#Canada">
        <rdfs:subClassOf rdf:resource="http://www.semanticweb.org/cassandwich/ontologies/2018/2/podcast-ontology#PodcastCountryOfOrigin"/>
        <rdfs:comment>Country of origin is Canada.</rdfs:comment>
    </owl:Class>
    


    <!-- http://www.semanticweb.org/cassandwich/ontologies/2018/2/podcast-ontology#CanadianTrueCrime -->

    <owl:Class rdf:about="http://www.semanticweb.org/cassandwich/ontologies/2018/2/podcast-ontology#CanadianTrueCrime">
        <rdfs:subClassOf rdf:resource="http://www.semanticweb.org/cassandwich/ontologies/2018/2/podcast-ontology#PodcastTitle"/>
        <rdfs:subClassOf>
            <owl:Restriction>
                <owl:onProperty rdf:resource="http://www.semanticweb.org/cassandwich/ontologies/2018/2/podcast-ontology#has_number_of_hosts"/>
                <owl:someValuesFrom rdf:resource="http://www.semanticweb.org/cassandwich/ontologies/2018/2/podcast-ontology#One"/>
            </owl:Restriction>
        </rdfs:subClassOf>
        <rdfs:subClassOf>
            <owl:Restriction>
                <owl:onProperty rdf:resource="http://www.semanticweb.org/cassandwich/ontologies/2018/2/podcast-ontology#is_categorized_as"/>
                <owl:allValuesFrom rdf:resource="http://www.semanticweb.org/cassandwich/ontologies/2018/2/podcast-ontology#History"/>
            </owl:Restriction>
        </rdfs:subClassOf>
        <rdfs:subClassOf>
            <owl:Restriction>
                <owl:onProperty rdf:resource="http://www.semanticweb.org/cassandwich/ontologies/2018/2/podcast-ontology#is_from_country"/>
                <owl:allValuesFrom rdf:resource="http://www.semanticweb.org/cassandwich/ontologies/2018/2/podcast-ontology#Canada"/>
            </owl:Restriction>
        </rdfs:subClassOf>
        <rdfs:subClassOf>
            <owl:Restriction>
                <owl:onProperty rdf:resource="http://www.semanticweb.org/cassandwich/ontologies/2018/2/podcast-ontology#is_genre"/>
                <owl:allValuesFrom rdf:resource="http://www.semanticweb.org/cassandwich/ontologies/2018/2/podcast-ontology#NonFiction"/>
            </owl:Restriction>
        </rdfs:subClassOf>
        <rdfs:comment>Podcast is titled &apos;Canadian True Crime&apos;.

Reference: https://itunes.apple.com/ca/podcast/canadian-true-crime/id1197095887?mt=2</rdfs:comment>
    </owl:Class>
    


    <!-- http://www.semanticweb.org/cassandwich/ontologies/2018/2/podcast-ontology#Casefile -->

    <owl:Class rdf:about="http://www.semanticweb.org/cassandwich/ontologies/2018/2/podcast-ontology#Casefile">
        <rdfs:subClassOf rdf:resource="http://www.semanticweb.org/cassandwich/ontologies/2018/2/podcast-ontology#PodcastTitle"/>
        <rdfs:subClassOf>
            <owl:Restriction>
                <owl:onProperty rdf:resource="http://www.semanticweb.org/cassandwich/ontologies/2018/2/podcast-ontology#has_number_of_hosts"/>
                <owl:someValuesFrom rdf:resource="http://www.semanticweb.org/cassandwich/ontologies/2018/2/podcast-ontology#One"/>
            </owl:Restriction>
        </rdfs:subClassOf>
        <rdfs:subClassOf>
            <owl:Restriction>
                <owl:onProperty rdf:resource="http://www.semanticweb.org/cassandwich/ontologies/2018/2/podcast-ontology#is_categorized_as"/>
                <owl:allValuesFrom rdf:resource="http://www.semanticweb.org/cassandwich/ontologies/2018/2/podcast-ontology#History"/>
            </owl:Restriction>
        </rdfs:subClassOf>
        <rdfs:subClassOf>
            <owl:Restriction>
                <owl:onProperty rdf:resource="http://www.semanticweb.org/cassandwich/ontologies/2018/2/podcast-ontology#is_from_country"/>
                <owl:allValuesFrom rdf:resource="http://www.semanticweb.org/cassandwich/ontologies/2018/2/podcast-ontology#Australia"/>
            </owl:Restriction>
        </rdfs:subClassOf>
        <rdfs:subClassOf>
            <owl:Restriction>
                <owl:onProperty rdf:resource="http://www.semanticweb.org/cassandwich/ontologies/2018/2/podcast-ontology#is_genre"/>
                <owl:allValuesFrom rdf:resource="http://www.semanticweb.org/cassandwich/ontologies/2018/2/podcast-ontology#NonFiction"/>
            </owl:Restriction>
        </rdfs:subClassOf>
        <rdfs:comment>Podcast is titled &apos;Casefile&apos;.

Reference: https://itunes.apple.com/ca/podcast/casefile-true-crime/id998568017?mt=2</rdfs:comment>
    </owl:Class>
    


    <!-- http://www.semanticweb.org/cassandwich/ontologies/2018/2/podcast-ontology#ColdCaseFiles -->

    <owl:Class rdf:about="http://www.semanticweb.org/cassandwich/ontologies/2018/2/podcast-ontology#ColdCaseFiles">
        <rdfs:subClassOf rdf:resource="http://www.semanticweb.org/cassandwich/ontologies/2018/2/podcast-ontology#PodcastTitle"/>
        <rdfs:subClassOf>
            <owl:Restriction>
                <owl:onProperty rdf:resource="http://www.semanticweb.org/cassandwich/ontologies/2018/2/podcast-ontology#has_number_of_hosts"/>
                <owl:someValuesFrom rdf:resource="http://www.semanticweb.org/cassandwich/ontologies/2018/2/podcast-ontology#Two"/>
            </owl:Restriction>
        </rdfs:subClassOf>
        <rdfs:subClassOf>
            <owl:Restriction>
                <owl:onProperty rdf:resource="http://www.semanticweb.org/cassandwich/ontologies/2018/2/podcast-ontology#is_categorized_as"/>
                <owl:allValuesFrom rdf:resource="http://www.semanticweb.org/cassandwich/ontologies/2018/2/podcast-ontology#News&amp;Politics"/>
            </owl:Restriction>
        </rdfs:subClassOf>
        <rdfs:subClassOf>
            <owl:Restriction>
                <owl:onProperty rdf:resource="http://www.semanticweb.org/cassandwich/ontologies/2018/2/podcast-ontology#is_from_country"/>
                <owl:allValuesFrom rdf:resource="http://www.semanticweb.org/cassandwich/ontologies/2018/2/podcast-ontology#UnitedStates"/>
            </owl:Restriction>
        </rdfs:subClassOf>
        <rdfs:subClassOf>
            <owl:Restriction>
                <owl:onProperty rdf:resource="http://www.semanticweb.org/cassandwich/ontologies/2018/2/podcast-ontology#is_genre"/>
                <owl:allValuesFrom rdf:resource="http://www.semanticweb.org/cassandwich/ontologies/2018/2/podcast-ontology#NonFiction"/>
            </owl:Restriction>
        </rdfs:subClassOf>
        <rdfs:comment>Podcast is titled &apos;Cold Case Files&apos;.

Reference: https://itunes.apple.com/ca/podcast/cold-case-files-the-podcast/id1241386674?mt=2</rdfs:comment>
    </owl:Class>
    


    <!-- http://www.semanticweb.org/cassandwich/ontologies/2018/2/podcast-ontology#Comedy -->

    <owl:Class rdf:about="http://www.semanticweb.org/cassandwich/ontologies/2018/2/podcast-ontology#Comedy">
        <rdfs:subClassOf rdf:resource="http://www.semanticweb.org/cassandwich/ontologies/2018/2/podcast-ontology#PodcastCategory"/>
        <rdfs:comment>The category defined by iTunes as Comedy.

Reference: https://itunes.apple.com/ca/genre/podcasts-comedy/id1303?mt=2</rdfs:comment>
    </owl:Class>
    


    <!-- http://www.semanticweb.org/cassandwich/ontologies/2018/2/podcast-ontology#DebtFreeIn30 -->

    <owl:Class rdf:about="http://www.semanticweb.org/cassandwich/ontologies/2018/2/podcast-ontology#DebtFreeIn30">
        <rdfs:subClassOf rdf:resource="http://www.semanticweb.org/cassandwich/ontologies/2018/2/podcast-ontology#PodcastTitle"/>
        <rdfs:subClassOf>
            <owl:Restriction>
                <owl:onProperty rdf:resource="http://www.semanticweb.org/cassandwich/ontologies/2018/2/podcast-ontology#has_number_of_hosts"/>
                <owl:someValuesFrom rdf:resource="http://www.semanticweb.org/cassandwich/ontologies/2018/2/podcast-ontology#Two"/>
            </owl:Restriction>
        </rdfs:subClassOf>
        <rdfs:subClassOf>
            <owl:Restriction>
                <owl:onProperty rdf:resource="http://www.semanticweb.org/cassandwich/ontologies/2018/2/podcast-ontology#is_genre"/>
                <owl:someValuesFrom rdf:resource="http://www.semanticweb.org/cassandwich/ontologies/2018/2/podcast-ontology#NonFiction"/>
            </owl:Restriction>
        </rdfs:subClassOf>
        <rdfs:subClassOf>
            <owl:Restriction>
                <owl:onProperty rdf:resource="http://www.semanticweb.org/cassandwich/ontologies/2018/2/podcast-ontology#is_categorized_as"/>
                <owl:allValuesFrom rdf:resource="http://www.semanticweb.org/cassandwich/ontologies/2018/2/podcast-ontology#Investing"/>
            </owl:Restriction>
        </rdfs:subClassOf>
        <rdfs:subClassOf>
            <owl:Restriction>
                <owl:onProperty rdf:resource="http://www.semanticweb.org/cassandwich/ontologies/2018/2/podcast-ontology#is_from_country"/>
                <owl:allValuesFrom rdf:resource="http://www.semanticweb.org/cassandwich/ontologies/2018/2/podcast-ontology#Canada"/>
            </owl:Restriction>
        </rdfs:subClassOf>
        <rdfs:comment>Podcast is titled &apos;Debt Free in 30&apos;.

Reference: https://itunes.apple.com/ca/podcast/debt-free-in-30/id914550159?mt=2</rdfs:comment>
    </owl:Class>
    


    <!-- http://www.semanticweb.org/cassandwich/ontologies/2018/2/podcast-ontology#Design -->

    <owl:Class rdf:about="http://www.semanticweb.org/cassandwich/ontologies/2018/2/podcast-ontology#Design">
        <rdfs:subClassOf rdf:resource="http://www.semanticweb.org/cassandwich/ontologies/2018/2/podcast-ontology#Arts"/>
        <rdfs:comment>The subcategory of the Arts category defined by iTunes as Design.

Reference: https://itunes.apple.com/ca/genre/podcasts-arts-design/id1402?mt=2</rdfs:comment>
    </owl:Class>
    


    <!-- http://www.semanticweb.org/cassandwich/ontologies/2018/2/podcast-ontology#DoneDisappeared -->

    <owl:Class rdf:about="http://www.semanticweb.org/cassandwich/ontologies/2018/2/podcast-ontology#DoneDisappeared">
        <rdfs:subClassOf rdf:resource="http://www.semanticweb.org/cassandwich/ontologies/2018/2/podcast-ontology#PodcastTitle"/>
        <rdfs:subClassOf>
            <owl:Restriction>
                <owl:onProperty rdf:resource="http://www.semanticweb.org/cassandwich/ontologies/2018/2/podcast-ontology#has_number_of_hosts"/>
                <owl:allValuesFrom rdf:resource="http://www.semanticweb.org/cassandwich/ontologies/2018/2/podcast-ontology#One"/>
            </owl:Restriction>
        </rdfs:subClassOf>
        <rdfs:subClassOf>
            <owl:Restriction>
                <owl:onProperty rdf:resource="http://www.semanticweb.org/cassandwich/ontologies/2018/2/podcast-ontology#is_categorized_as"/>
                <owl:allValuesFrom rdf:resource="http://www.semanticweb.org/cassandwich/ontologies/2018/2/podcast-ontology#SocialSciences"/>
            </owl:Restriction>
        </rdfs:subClassOf>
        <rdfs:subClassOf>
            <owl:Restriction>
                <owl:onProperty rdf:resource="http://www.semanticweb.org/cassandwich/ontologies/2018/2/podcast-ontology#is_from_country"/>
                <owl:allValuesFrom rdf:resource="http://www.semanticweb.org/cassandwich/ontologies/2018/2/podcast-ontology#UnitedStates"/>
            </owl:Restriction>
        </rdfs:subClassOf>
        <rdfs:subClassOf>
            <owl:Restriction>
                <owl:onProperty rdf:resource="http://www.semanticweb.org/cassandwich/ontologies/2018/2/podcast-ontology#is_genre"/>
                <owl:allValuesFrom rdf:resource="http://www.semanticweb.org/cassandwich/ontologies/2018/2/podcast-ontology#Fiction"/>
            </owl:Restriction>
        </rdfs:subClassOf>
        <rdfs:comment>Podcast is titled &apos;Done Disappeared&apos;.

Reference: https://itunes.apple.com/ca/podcast/done-disappeared/id1301190222?mt=2</rdfs:comment>
    </owl:Class>
    


    <!-- http://www.semanticweb.org/cassandwich/ontologies/2018/2/podcast-ontology#Doughboys -->

    <owl:Class rdf:about="http://www.semanticweb.org/cassandwich/ontologies/2018/2/podcast-ontology#Doughboys">
        <rdfs:subClassOf rdf:resource="http://www.semanticweb.org/cassandwich/ontologies/2018/2/podcast-ontology#PodcastTitle"/>
        <rdfs:subClassOf>
            <owl:Restriction>
                <owl:onProperty rdf:resource="http://www.semanticweb.org/cassandwich/ontologies/2018/2/podcast-ontology#has_number_of_hosts"/>
                <owl:someValuesFrom rdf:resource="http://www.semanticweb.org/cassandwich/ontologies/2018/2/podcast-ontology#Two"/>
            </owl:Restriction>
        </rdfs:subClassOf>
        <rdfs:subClassOf>
            <owl:Restriction>
                <owl:onProperty rdf:resource="http://www.semanticweb.org/cassandwich/ontologies/2018/2/podcast-ontology#is_genre"/>
                <owl:someValuesFrom rdf:resource="http://www.semanticweb.org/cassandwich/ontologies/2018/2/podcast-ontology#NonFiction"/>
            </owl:Restriction>
        </rdfs:subClassOf>
        <rdfs:subClassOf>
            <owl:Restriction>
                <owl:onProperty rdf:resource="http://www.semanticweb.org/cassandwich/ontologies/2018/2/podcast-ontology#is_categorized_as"/>
                <owl:allValuesFrom rdf:resource="http://www.semanticweb.org/cassandwich/ontologies/2018/2/podcast-ontology#Comedy"/>
            </owl:Restriction>
        </rdfs:subClassOf>
        <rdfs:subClassOf>
            <owl:Restriction>
                <owl:onProperty rdf:resource="http://www.semanticweb.org/cassandwich/ontologies/2018/2/podcast-ontology#is_from_country"/>
                <owl:allValuesFrom rdf:resource="http://www.semanticweb.org/cassandwich/ontologies/2018/2/podcast-ontology#UnitedStates"/>
            </owl:Restriction>
        </rdfs:subClassOf>
        <rdfs:comment>Podcast is titled &apos;Doughboys&apos;.

Reference: https://itunes.apple.com/ca/podcast/doughboys/id996151267?mt=2</rdfs:comment>
    </owl:Class>
    


    <!-- http://www.semanticweb.org/cassandwich/ontologies/2018/2/podcast-ontology#Education -->

    <owl:Class rdf:about="http://www.semanticweb.org/cassandwich/ontologies/2018/2/podcast-ontology#Education">
        <rdfs:subClassOf rdf:resource="http://www.semanticweb.org/cassandwich/ontologies/2018/2/podcast-ontology#PodcastCategory"/>
        <rdfs:comment>The category defined by iTunes as Education.

Reference: https://itunes.apple.com/ca/genre/podcasts-education/id1304?mt=2</rdfs:comment>
    </owl:Class>
    


    <!-- http://www.semanticweb.org/cassandwich/ontologies/2018/2/podcast-ontology#England -->

    <owl:Class rdf:about="http://www.semanticweb.org/cassandwich/ontologies/2018/2/podcast-ontology#England">
        <rdfs:subClassOf rdf:resource="http://www.semanticweb.org/cassandwich/ontologies/2018/2/podcast-ontology#PodcastCountryOfOrigin"/>
        <rdfs:comment>Country of origin is England.</rdfs:comment>
    </owl:Class>
    


    <!-- http://www.semanticweb.org/cassandwich/ontologies/2018/2/podcast-ontology#FaultLines -->

    <owl:Class rdf:about="http://www.semanticweb.org/cassandwich/ontologies/2018/2/podcast-ontology#FaultLines">
        <rdfs:subClassOf rdf:resource="http://www.semanticweb.org/cassandwich/ontologies/2018/2/podcast-ontology#PodcastTitle"/>
        <rdfs:subClassOf>
            <owl:Restriction>
                <owl:onProperty rdf:resource="http://www.semanticweb.org/cassandwich/ontologies/2018/2/podcast-ontology#is_genre"/>
                <owl:someValuesFrom rdf:resource="http://www.semanticweb.org/cassandwich/ontologies/2018/2/podcast-ontology#NonFiction"/>
            </owl:Restriction>
        </rdfs:subClassOf>
        <rdfs:subClassOf>
            <owl:Restriction>
                <owl:onProperty rdf:resource="http://www.semanticweb.org/cassandwich/ontologies/2018/2/podcast-ontology#has_number_of_hosts"/>
                <owl:allValuesFrom rdf:resource="http://www.semanticweb.org/cassandwich/ontologies/2018/2/podcast-ontology#One"/>
            </owl:Restriction>
        </rdfs:subClassOf>
        <rdfs:subClassOf>
            <owl:Restriction>
                <owl:onProperty rdf:resource="http://www.semanticweb.org/cassandwich/ontologies/2018/2/podcast-ontology#is_categorized_as"/>
                <owl:allValuesFrom rdf:resource="http://www.semanticweb.org/cassandwich/ontologies/2018/2/podcast-ontology#Society&amp;Culture"/>
            </owl:Restriction>
        </rdfs:subClassOf>
        <rdfs:subClassOf>
            <owl:Restriction>
                <owl:onProperty rdf:resource="http://www.semanticweb.org/cassandwich/ontologies/2018/2/podcast-ontology#is_from_country"/>
                <owl:allValuesFrom rdf:resource="http://www.semanticweb.org/cassandwich/ontologies/2018/2/podcast-ontology#Canada"/>
            </owl:Restriction>
        </rdfs:subClassOf>
        <rdfs:comment>Podcast is titled &apos;Fault Lines&apos;.

Reference: https://itunes.apple.com/ca/podcast/fault-lines/id1162124786?mt=2</rdfs:comment>
    </owl:Class>
    


    <!-- http://www.semanticweb.org/cassandwich/ontologies/2018/2/podcast-ontology#Fiction -->

    <owl:Class rdf:about="http://www.semanticweb.org/cassandwich/ontologies/2018/2/podcast-ontology#Fiction">
        <rdfs:subClassOf rdf:resource="http://www.semanticweb.org/cassandwich/ontologies/2018/2/podcast-ontology#Genre"/>
        <owl:disjointWith rdf:resource="http://www.semanticweb.org/cassandwich/ontologies/2018/2/podcast-ontology#NonFiction"/>
        <rdfs:comment>Fiction is something feigned, invented, or imagined; a made-up story.

Reference: http://www.dictionary.com/browse/fiction</rdfs:comment>
    </owl:Class>
    


    <!-- http://www.semanticweb.org/cassandwich/ontologies/2018/2/podcast-ontology#Five -->

    <owl:Class rdf:about="http://www.semanticweb.org/cassandwich/ontologies/2018/2/podcast-ontology#Five">
        <rdfs:subClassOf rdf:resource="http://www.semanticweb.org/cassandwich/ontologies/2018/2/podcast-ontology#NumberOfHosts"/>
        <rdfs:comment>Five individuals as hosts.</rdfs:comment>
    </owl:Class>
    


    <!-- http://www.semanticweb.org/cassandwich/ontologies/2018/2/podcast-ontology#Four -->

    <owl:Class rdf:about="http://www.semanticweb.org/cassandwich/ontologies/2018/2/podcast-ontology#Four">
        <rdfs:subClassOf rdf:resource="http://www.semanticweb.org/cassandwich/ontologies/2018/2/podcast-ontology#NumberOfHosts"/>
        <rdfs:comment>Four individuals as hosts.</rdfs:comment>
    </owl:Class>
    


    <!-- http://www.semanticweb.org/cassandwich/ontologies/2018/2/podcast-ontology#FreakonomicsRadio -->

    <owl:Class rdf:about="http://www.semanticweb.org/cassandwich/ontologies/2018/2/podcast-ontology#FreakonomicsRadio">
        <rdfs:subClassOf rdf:resource="http://www.semanticweb.org/cassandwich/ontologies/2018/2/podcast-ontology#PodcastTitle"/>
        <rdfs:subClassOf>
            <owl:Restriction>
                <owl:onProperty rdf:resource="http://www.semanticweb.org/cassandwich/ontologies/2018/2/podcast-ontology#has_number_of_hosts"/>
                <owl:someValuesFrom rdf:resource="http://www.semanticweb.org/cassandwich/ontologies/2018/2/podcast-ontology#Two"/>
            </owl:Restriction>
        </rdfs:subClassOf>
        <rdfs:subClassOf>
            <owl:Restriction>
                <owl:onProperty rdf:resource="http://www.semanticweb.org/cassandwich/ontologies/2018/2/podcast-ontology#is_genre"/>
                <owl:someValuesFrom rdf:resource="http://www.semanticweb.org/cassandwich/ontologies/2018/2/podcast-ontology#NonFiction"/>
            </owl:Restriction>
        </rdfs:subClassOf>
        <rdfs:subClassOf>
            <owl:Restriction>
                <owl:onProperty rdf:resource="http://www.semanticweb.org/cassandwich/ontologies/2018/2/podcast-ontology#is_categorized_as"/>
                <owl:allValuesFrom rdf:resource="http://www.semanticweb.org/cassandwich/ontologies/2018/2/podcast-ontology#Society&amp;Culture"/>
            </owl:Restriction>
        </rdfs:subClassOf>
        <rdfs:subClassOf>
            <owl:Restriction>
                <owl:onProperty rdf:resource="http://www.semanticweb.org/cassandwich/ontologies/2018/2/podcast-ontology#is_from_country"/>
                <owl:allValuesFrom rdf:resource="http://www.semanticweb.org/cassandwich/ontologies/2018/2/podcast-ontology#UnitedStates"/>
            </owl:Restriction>
        </rdfs:subClassOf>
        <rdfs:comment>Podcast is titled &apos;Freakonomics Radio&apos;.

Reference: https://itunes.apple.com/ca/podcast/freakonomics-radio/id354668519?mt=2</rdfs:comment>
    </owl:Class>
    


    <!-- http://www.semanticweb.org/cassandwich/ontologies/2018/2/podcast-ontology#Genre -->

    <owl:Class rdf:about="http://www.semanticweb.org/cassandwich/ontologies/2018/2/podcast-ontology#Genre">
        <rdfs:comment>The genre of the podcast content.</rdfs:comment>
    </owl:Class>
    


    <!-- http://www.semanticweb.org/cassandwich/ontologies/2018/2/podcast-ontology#HarryPotterAndTheSacredText -->

    <owl:Class rdf:about="http://www.semanticweb.org/cassandwich/ontologies/2018/2/podcast-ontology#HarryPotterAndTheSacredText">
        <rdfs:subClassOf rdf:resource="http://www.semanticweb.org/cassandwich/ontologies/2018/2/podcast-ontology#PodcastTitle"/>
        <rdfs:subClassOf>
            <owl:Restriction>
                <owl:onProperty rdf:resource="http://www.semanticweb.org/cassandwich/ontologies/2018/2/podcast-ontology#has_number_of_hosts"/>
                <owl:someValuesFrom rdf:resource="http://www.semanticweb.org/cassandwich/ontologies/2018/2/podcast-ontology#Two"/>
            </owl:Restriction>
        </rdfs:subClassOf>
        <rdfs:subClassOf>
            <owl:Restriction>
                <owl:onProperty rdf:resource="http://www.semanticweb.org/cassandwich/ontologies/2018/2/podcast-ontology#is_genre"/>
                <owl:someValuesFrom rdf:resource="http://www.semanticweb.org/cassandwich/ontologies/2018/2/podcast-ontology#NonFiction"/>
            </owl:Restriction>
        </rdfs:subClassOf>
        <rdfs:subClassOf>
            <owl:Restriction>
                <owl:onProperty rdf:resource="http://www.semanticweb.org/cassandwich/ontologies/2018/2/podcast-ontology#is_categorized_as"/>
                <owl:allValuesFrom rdf:resource="http://www.semanticweb.org/cassandwich/ontologies/2018/2/podcast-ontology#Religion&amp;Spirituality"/>
            </owl:Restriction>
        </rdfs:subClassOf>
        <rdfs:subClassOf>
            <owl:Restriction>
                <owl:onProperty rdf:resource="http://www.semanticweb.org/cassandwich/ontologies/2018/2/podcast-ontology#is_from_country"/>
                <owl:allValuesFrom rdf:resource="http://www.semanticweb.org/cassandwich/ontologies/2018/2/podcast-ontology#UnitedStates"/>
            </owl:Restriction>
        </rdfs:subClassOf>
        <rdfs:comment>Podcast is titled &apos;Harry Potter and the Sacred Text&apos;.

Reference: https://itunes.apple.com/ca/podcast/harry-potter-and-the-sacred-text/id1096113994?mt=2</rdfs:comment>
    </owl:Class>
    


    <!-- http://www.semanticweb.org/cassandwich/ontologies/2018/2/podcast-ontology#Health -->

    <owl:Class rdf:about="http://www.semanticweb.org/cassandwich/ontologies/2018/2/podcast-ontology#Health">
        <rdfs:subClassOf rdf:resource="http://www.semanticweb.org/cassandwich/ontologies/2018/2/podcast-ontology#PodcastCategory"/>
        <rdfs:comment>The category defined by iTunes as Health.

Reference: https://itunes.apple.com/ca/genre/podcasts-health/id1307?mt=2</rdfs:comment>
    </owl:Class>
    


    <!-- http://www.semanticweb.org/cassandwich/ontologies/2018/2/podcast-ontology#HeavensGate -->

    <owl:Class rdf:about="http://www.semanticweb.org/cassandwich/ontologies/2018/2/podcast-ontology#HeavensGate">
        <rdfs:subClassOf rdf:resource="http://www.semanticweb.org/cassandwich/ontologies/2018/2/podcast-ontology#PodcastTitle"/>
        <rdfs:subClassOf>
            <owl:Restriction>
                <owl:onProperty rdf:resource="http://www.semanticweb.org/cassandwich/ontologies/2018/2/podcast-ontology#has_number_of_hosts"/>
                <owl:allValuesFrom rdf:resource="http://www.semanticweb.org/cassandwich/ontologies/2018/2/podcast-ontology#One"/>
            </owl:Restriction>
        </rdfs:subClassOf>
        <rdfs:subClassOf>
            <owl:Restriction>
                <owl:onProperty rdf:resource="http://www.semanticweb.org/cassandwich/ontologies/2018/2/podcast-ontology#is_categorized_as"/>
                <owl:allValuesFrom rdf:resource="http://www.semanticweb.org/cassandwich/ontologies/2018/2/podcast-ontology#History"/>
            </owl:Restriction>
        </rdfs:subClassOf>
        <rdfs:subClassOf>
            <owl:Restriction>
                <owl:onProperty rdf:resource="http://www.semanticweb.org/cassandwich/ontologies/2018/2/podcast-ontology#is_from_country"/>
                <owl:allValuesFrom rdf:resource="http://www.semanticweb.org/cassandwich/ontologies/2018/2/podcast-ontology#UnitedStates"/>
            </owl:Restriction>
        </rdfs:subClassOf>
        <rdfs:subClassOf>
            <owl:Restriction>
                <owl:onProperty rdf:resource="http://www.semanticweb.org/cassandwich/ontologies/2018/2/podcast-ontology#is_genre"/>
                <owl:allValuesFrom rdf:resource="http://www.semanticweb.org/cassandwich/ontologies/2018/2/podcast-ontology#NonFiction"/>
            </owl:Restriction>
        </rdfs:subClassOf>
        <rdfs:comment>Podcast is titled &apos;Heaven&apos;s Gate&apos;.

Reference: https://itunes.apple.com/ca/podcast/heavens-gate/id1292069401?mt=2</rdfs:comment>
    </owl:Class>
    


    <!-- http://www.semanticweb.org/cassandwich/ontologies/2018/2/podcast-ontology#History -->

    <owl:Class rdf:about="http://www.semanticweb.org/cassandwich/ontologies/2018/2/podcast-ontology#History">
        <rdfs:subClassOf rdf:resource="http://www.semanticweb.org/cassandwich/ontologies/2018/2/podcast-ontology#Society&amp;Culture"/>
        <owl:disjointWith rdf:resource="http://www.semanticweb.org/cassandwich/ontologies/2018/2/podcast-ontology#Philosophy"/>
        <rdfs:comment>The subcategory of the Society &amp; Culture category defined by iTunes as History.

Reference: https://itunes.apple.com/ca/genre/podcasts-society-culture-history/id1462?mt=2</rdfs:comment>
    </owl:Class>
    


    <!-- http://www.semanticweb.org/cassandwich/ontologies/2018/2/podcast-ontology#Hobbies -->

    <owl:Class rdf:about="http://www.semanticweb.org/cassandwich/ontologies/2018/2/podcast-ontology#Hobbies">
        <rdfs:subClassOf rdf:resource="http://www.semanticweb.org/cassandwich/ontologies/2018/2/podcast-ontology#Games&amp;Hobbies"/>
        <rdfs:comment>The subcategory of the Games &amp; Hobbies category defined by iTunes as Hobbies.

Reference: https://itunes.apple.com/ca/genre/podcasts-games-hobbies-hobbies/id1460?mt=2</rdfs:comment>
    </owl:Class>
    


    <!-- http://www.semanticweb.org/cassandwich/ontologies/2018/2/podcast-ontology#HowDidThisGetMade -->

    <owl:Class rdf:about="http://www.semanticweb.org/cassandwich/ontologies/2018/2/podcast-ontology#HowDidThisGetMade">
        <rdfs:subClassOf rdf:resource="http://www.semanticweb.org/cassandwich/ontologies/2018/2/podcast-ontology#PodcastTitle"/>
        <rdfs:subClassOf>
            <owl:Restriction>
                <owl:onProperty rdf:resource="http://www.semanticweb.org/cassandwich/ontologies/2018/2/podcast-ontology#has_number_of_hosts"/>
                <owl:someValuesFrom rdf:resource="http://www.semanticweb.org/cassandwich/ontologies/2018/2/podcast-ontology#Three"/>
            </owl:Restriction>
        </rdfs:subClassOf>
        <rdfs:subClassOf>
            <owl:Restriction>
                <owl:onProperty rdf:resource="http://www.semanticweb.org/cassandwich/ontologies/2018/2/podcast-ontology#is_categorized_as"/>
                <owl:allValuesFrom rdf:resource="http://www.semanticweb.org/cassandwich/ontologies/2018/2/podcast-ontology#Comedy"/>
            </owl:Restriction>
        </rdfs:subClassOf>
        <rdfs:subClassOf>
            <owl:Restriction>
                <owl:onProperty rdf:resource="http://www.semanticweb.org/cassandwich/ontologies/2018/2/podcast-ontology#is_from_country"/>
                <owl:allValuesFrom rdf:resource="http://www.semanticweb.org/cassandwich/ontologies/2018/2/podcast-ontology#UnitedStates"/>
            </owl:Restriction>
        </rdfs:subClassOf>
        <rdfs:subClassOf>
            <owl:Restriction>
                <owl:onProperty rdf:resource="http://www.semanticweb.org/cassandwich/ontologies/2018/2/podcast-ontology#is_genre"/>
                <owl:allValuesFrom rdf:resource="http://www.semanticweb.org/cassandwich/ontologies/2018/2/podcast-ontology#NonFiction"/>
            </owl:Restriction>
        </rdfs:subClassOf>
        <rdfs:comment>Podcast is titled &apos;How Did This Get Made&apos;.

Reference: https://itunes.apple.com/ca/podcast/how-did-this-get-made/id409287913?mt=2</rdfs:comment>
    </owl:Class>
    


    <!-- http://www.semanticweb.org/cassandwich/ontologies/2018/2/podcast-ontology#Investing -->

    <owl:Class rdf:about="http://www.semanticweb.org/cassandwich/ontologies/2018/2/podcast-ontology#Investing">
        <rdfs:subClassOf rdf:resource="http://www.semanticweb.org/cassandwich/ontologies/2018/2/podcast-ontology#Business"/>
        <rdfs:comment>The subcategory of the Business category defined by iTunes as Investing.

Reference: https://itunes.apple.com/ca/genre/podcasts-business-investing/id1412?mt=2</rdfs:comment>
    </owl:Class>
    


    <!-- http://www.semanticweb.org/cassandwich/ontologies/2018/2/podcast-ontology#KnitPicksPodcast -->

    <owl:Class rdf:about="http://www.semanticweb.org/cassandwich/ontologies/2018/2/podcast-ontology#KnitPicksPodcast">
        <rdfs:subClassOf rdf:resource="http://www.semanticweb.org/cassandwich/ontologies/2018/2/podcast-ontology#PodcastTitle"/>
        <rdfs:subClassOf>
            <owl:Restriction>
                <owl:onProperty rdf:resource="http://www.semanticweb.org/cassandwich/ontologies/2018/2/podcast-ontology#is_categorized_as"/>
                <owl:allValuesFrom rdf:resource="http://www.semanticweb.org/cassandwich/ontologies/2018/2/podcast-ontology#Hobbies"/>
            </owl:Restriction>
        </rdfs:subClassOf>
        <rdfs:subClassOf>
            <owl:Restriction>
                <owl:onProperty rdf:resource="http://www.semanticweb.org/cassandwich/ontologies/2018/2/podcast-ontology#is_from_country"/>
                <owl:allValuesFrom rdf:resource="http://www.semanticweb.org/cassandwich/ontologies/2018/2/podcast-ontology#UnitedStates"/>
            </owl:Restriction>
        </rdfs:subClassOf>
        <rdfs:subClassOf>
            <owl:Restriction>
                <owl:onProperty rdf:resource="http://www.semanticweb.org/cassandwich/ontologies/2018/2/podcast-ontology#is_genre"/>
                <owl:allValuesFrom rdf:resource="http://www.semanticweb.org/cassandwich/ontologies/2018/2/podcast-ontology#NonFiction"/>
            </owl:Restriction>
        </rdfs:subClassOf>
        <rdfs:subClassOf>
            <owl:Restriction>
                <owl:onProperty rdf:resource="http://www.semanticweb.org/cassandwich/ontologies/2018/2/podcast-ontology#has_number_of_hosts"/>
                <owl:minQualifiedCardinality rdf:datatype="http://www.w3.org/2001/XMLSchema#nonNegativeInteger">1</owl:minQualifiedCardinality>
                <owl:onClass rdf:resource="http://www.semanticweb.org/cassandwich/ontologies/2018/2/podcast-ontology#One"/>
            </owl:Restriction>
        </rdfs:subClassOf>
        <rdfs:comment>Podcast is titled &apos;Knit Picks Podcast&apos;.

Reference: https://itunes.apple.com/ca/podcast/knit-picks-podcast/id253212700?mt=2</rdfs:comment>
    </owl:Class>
    


    <!-- http://www.semanticweb.org/cassandwich/ontologies/2018/2/podcast-ontology#Music -->

    <owl:Class rdf:about="http://www.semanticweb.org/cassandwich/ontologies/2018/2/podcast-ontology#Music">
        <rdfs:subClassOf rdf:resource="http://www.semanticweb.org/cassandwich/ontologies/2018/2/podcast-ontology#PodcastCategory"/>
        <rdfs:comment>The category defined by iTunes as Music.

Reference: https://itunes.apple.com/ca/genre/podcasts-music/id1310?mt=2</rdfs:comment>
    </owl:Class>
    


    <!-- http://www.semanticweb.org/cassandwich/ontologies/2018/2/podcast-ontology#MyFavoriteMurder -->

    <owl:Class rdf:about="http://www.semanticweb.org/cassandwich/ontologies/2018/2/podcast-ontology#MyFavoriteMurder">
        <rdfs:subClassOf rdf:resource="http://www.semanticweb.org/cassandwich/ontologies/2018/2/podcast-ontology#PodcastTitle"/>
        <rdfs:subClassOf>
            <owl:Restriction>
                <owl:onProperty rdf:resource="http://www.semanticweb.org/cassandwich/ontologies/2018/2/podcast-ontology#is_genre"/>
                <owl:someValuesFrom rdf:resource="http://www.semanticweb.org/cassandwich/ontologies/2018/2/podcast-ontology#NonFiction"/>
            </owl:Restriction>
        </rdfs:subClassOf>
        <rdfs:subClassOf>
            <owl:Restriction>
                <owl:onProperty rdf:resource="http://www.semanticweb.org/cassandwich/ontologies/2018/2/podcast-ontology#has_number_of_hosts"/>
                <owl:allValuesFrom rdf:resource="http://www.semanticweb.org/cassandwich/ontologies/2018/2/podcast-ontology#Two"/>
            </owl:Restriction>
        </rdfs:subClassOf>
        <rdfs:subClassOf>
            <owl:Restriction>
                <owl:onProperty rdf:resource="http://www.semanticweb.org/cassandwich/ontologies/2018/2/podcast-ontology#is_categorized_as"/>
                <owl:allValuesFrom rdf:resource="http://www.semanticweb.org/cassandwich/ontologies/2018/2/podcast-ontology#Comedy"/>
            </owl:Restriction>
        </rdfs:subClassOf>
        <rdfs:subClassOf>
            <owl:Restriction>
                <owl:onProperty rdf:resource="http://www.semanticweb.org/cassandwich/ontologies/2018/2/podcast-ontology#is_from_country"/>
                <owl:allValuesFrom rdf:resource="http://www.semanticweb.org/cassandwich/ontologies/2018/2/podcast-ontology#UnitedStates"/>
            </owl:Restriction>
        </rdfs:subClassOf>
        <rdfs:comment>Podcast is titled &apos;My Favorite Murder&apos;.

Reference: https://itunes.apple.com/us/podcast/my-favorite-murder-karen-kilgariff-georgia-hardstark/id1074507850?mt=2</rdfs:comment>
    </owl:Class>
    


    <!-- http://www.semanticweb.org/cassandwich/ontologies/2018/2/podcast-ontology#NaturalSciences -->

    <owl:Class rdf:about="http://www.semanticweb.org/cassandwich/ontologies/2018/2/podcast-ontology#NaturalSciences">
        <rdfs:subClassOf rdf:resource="http://www.semanticweb.org/cassandwich/ontologies/2018/2/podcast-ontology#Science&amp;Medicine"/>
        <rdfs:comment>The subcategory of the Science &amp; Medicine category defined by iTunes as Natural Sciences.

Reference: https://itunes.apple.com/ca/genre/podcasts-science-medicine-natural-sciences/id1477?mt=2</rdfs:comment>
    </owl:Class>
    


    <!-- http://www.semanticweb.org/cassandwich/ontologies/2018/2/podcast-ontology#NewZealand -->

    <owl:Class rdf:about="http://www.semanticweb.org/cassandwich/ontologies/2018/2/podcast-ontology#NewZealand">
        <rdfs:subClassOf rdf:resource="http://www.semanticweb.org/cassandwich/ontologies/2018/2/podcast-ontology#PodcastCountryOfOrigin"/>
        <rdfs:comment>Country of origin is New Zealand.</rdfs:comment>
    </owl:Class>
    


    <!-- http://www.semanticweb.org/cassandwich/ontologies/2018/2/podcast-ontology#NightTime -->

    <owl:Class rdf:about="http://www.semanticweb.org/cassandwich/ontologies/2018/2/podcast-ontology#NightTime">
        <rdfs:subClassOf rdf:resource="http://www.semanticweb.org/cassandwich/ontologies/2018/2/podcast-ontology#PodcastTitle"/>
        <rdfs:subClassOf>
            <owl:Restriction>
                <owl:onProperty rdf:resource="http://www.semanticweb.org/cassandwich/ontologies/2018/2/podcast-ontology#has_number_of_hosts"/>
                <owl:allValuesFrom rdf:resource="http://www.semanticweb.org/cassandwich/ontologies/2018/2/podcast-ontology#One"/>
            </owl:Restriction>
        </rdfs:subClassOf>
        <rdfs:subClassOf>
            <owl:Restriction>
                <owl:onProperty rdf:resource="http://www.semanticweb.org/cassandwich/ontologies/2018/2/podcast-ontology#is_categorized_as"/>
                <owl:allValuesFrom rdf:resource="http://www.semanticweb.org/cassandwich/ontologies/2018/2/podcast-ontology#PersonalJournals"/>
            </owl:Restriction>
        </rdfs:subClassOf>
        <rdfs:subClassOf>
            <owl:Restriction>
                <owl:onProperty rdf:resource="http://www.semanticweb.org/cassandwich/ontologies/2018/2/podcast-ontology#is_from_country"/>
                <owl:allValuesFrom rdf:resource="http://www.semanticweb.org/cassandwich/ontologies/2018/2/podcast-ontology#Canada"/>
            </owl:Restriction>
        </rdfs:subClassOf>
        <rdfs:subClassOf>
            <owl:Restriction>
                <owl:onProperty rdf:resource="http://www.semanticweb.org/cassandwich/ontologies/2018/2/podcast-ontology#is_genre"/>
                <owl:allValuesFrom rdf:resource="http://www.semanticweb.org/cassandwich/ontologies/2018/2/podcast-ontology#NonFiction"/>
            </owl:Restriction>
        </rdfs:subClassOf>
        <rdfs:comment>Podcast is titled &apos;Night Time&apos;.

Reference: https://itunes.apple.com/ca/podcast/nighttime-canadian-crime-mysteries-and-the-weird/id1054220508?mt=2</rdfs:comment>
    </owl:Class>
    


    <!-- http://www.semanticweb.org/cassandwich/ontologies/2018/2/podcast-ontology#NonFiction -->

    <owl:Class rdf:about="http://www.semanticweb.org/cassandwich/ontologies/2018/2/podcast-ontology#NonFiction">
        <rdfs:subClassOf rdf:resource="http://www.semanticweb.org/cassandwich/ontologies/2018/2/podcast-ontology#Genre"/>
        <rdfs:comment>Something that is about facts and real events.

Reference: https://www.merriam-webster.com/dictionary/nonfiction</rdfs:comment>
    </owl:Class>
    


    <!-- http://www.semanticweb.org/cassandwich/ontologies/2018/2/podcast-ontology#NumberOfHosts -->

    <owl:Class rdf:about="http://www.semanticweb.org/cassandwich/ontologies/2018/2/podcast-ontology#NumberOfHosts">
        <rdfs:comment>The number of hosts of the podcast.</rdfs:comment>
    </owl:Class>
    


    <!-- http://www.semanticweb.org/cassandwich/ontologies/2018/2/podcast-ontology#One -->

    <owl:Class rdf:about="http://www.semanticweb.org/cassandwich/ontologies/2018/2/podcast-ontology#One">
        <rdfs:subClassOf rdf:resource="http://www.semanticweb.org/cassandwich/ontologies/2018/2/podcast-ontology#NumberOfHosts"/>
        <rdfs:comment>One individual as host.</rdfs:comment>
    </owl:Class>
    


    <!-- http://www.semanticweb.org/cassandwich/ontologies/2018/2/podcast-ontology#PerformingArts -->

    <owl:Class rdf:about="http://www.semanticweb.org/cassandwich/ontologies/2018/2/podcast-ontology#PerformingArts">
        <rdfs:subClassOf rdf:resource="http://www.semanticweb.org/cassandwich/ontologies/2018/2/podcast-ontology#Arts"/>
        <rdfs:comment>The subcategory of the Arts category defined by iTunes as Performing Arts.

Reference: https://itunes.apple.com/ca/genre/podcasts-arts-performing-arts/id1405?mt=2</rdfs:comment>
    </owl:Class>
    


    <!-- http://www.semanticweb.org/cassandwich/ontologies/2018/2/podcast-ontology#PersonalJournals -->

    <owl:Class rdf:about="http://www.semanticweb.org/cassandwich/ontologies/2018/2/podcast-ontology#PersonalJournals">
        <rdfs:subClassOf rdf:resource="http://www.semanticweb.org/cassandwich/ontologies/2018/2/podcast-ontology#Society&amp;Culture"/>
        <rdfs:comment>The subcategory of the Society &amp; Culture category defined by iTunes as Personal Journals.

Reference: https://itunes.apple.com/ca/genre/podcasts-society-culture-personal-journals/id1302?mt=2</rdfs:comment>
    </owl:Class>
    


    <!-- http://www.semanticweb.org/cassandwich/ontologies/2018/2/podcast-ontology#Philosophy -->

    <owl:Class rdf:about="http://www.semanticweb.org/cassandwich/ontologies/2018/2/podcast-ontology#Philosophy">
        <rdfs:subClassOf rdf:resource="http://www.semanticweb.org/cassandwich/ontologies/2018/2/podcast-ontology#Society&amp;Culture"/>
        <rdfs:subClassOf>
            <owl:Restriction>
                <owl:onProperty rdf:resource="http://www.semanticweb.org/cassandwich/ontologies/2018/2/podcast-ontology#has_number_of_hosts"/>
                <owl:someValuesFrom rdf:resource="http://www.semanticweb.org/cassandwich/ontologies/2018/2/podcast-ontology#Two"/>
            </owl:Restriction>
        </rdfs:subClassOf>
        <rdfs:subClassOf>
            <owl:Restriction>
                <owl:onProperty rdf:resource="http://www.semanticweb.org/cassandwich/ontologies/2018/2/podcast-ontology#is_genre"/>
                <owl:someValuesFrom rdf:resource="http://www.semanticweb.org/cassandwich/ontologies/2018/2/podcast-ontology#NonFiction"/>
            </owl:Restriction>
        </rdfs:subClassOf>
        <rdfs:subClassOf>
            <owl:Restriction>
                <owl:onProperty rdf:resource="http://www.semanticweb.org/cassandwich/ontologies/2018/2/podcast-ontology#is_categorized_as"/>
                <owl:allValuesFrom rdf:resource="http://www.semanticweb.org/cassandwich/ontologies/2018/2/podcast-ontology#Philosophy"/>
            </owl:Restriction>
        </rdfs:subClassOf>
        <rdfs:subClassOf>
            <owl:Restriction>
                <owl:onProperty rdf:resource="http://www.semanticweb.org/cassandwich/ontologies/2018/2/podcast-ontology#is_from_country"/>
                <owl:allValuesFrom rdf:resource="http://www.semanticweb.org/cassandwich/ontologies/2018/2/podcast-ontology#UnitedStates"/>
            </owl:Restriction>
        </rdfs:subClassOf>
        <rdfs:comment>The subcategory of the Society &amp; Culture category defined by iTunes as Philosophy.

Reference: https://itunes.apple.com/ca/genre/podcasts-society-culture-philosophy/id1443?mt=2</rdfs:comment>
    </owl:Class>
    


    <!-- http://www.semanticweb.org/cassandwich/ontologies/2018/2/podcast-ontology#PodcastCategory -->

    <owl:Class rdf:about="http://www.semanticweb.org/cassandwich/ontologies/2018/2/podcast-ontology#PodcastCategory">
        <rdfs:comment>The category the podcast is classified as in the iTunes podcast charts.

Reference: https://castos.com/itunes-podcast-category-list/</rdfs:comment>
    </owl:Class>
    


    <!-- http://www.semanticweb.org/cassandwich/ontologies/2018/2/podcast-ontology#PodcastCountryOfOrigin -->

    <owl:Class rdf:about="http://www.semanticweb.org/cassandwich/ontologies/2018/2/podcast-ontology#PodcastCountryOfOrigin">
        <rdfs:comment>The country from which the podcast is recorded and distributed.</rdfs:comment>
    </owl:Class>
    


    <!-- http://www.semanticweb.org/cassandwich/ontologies/2018/2/podcast-ontology#PodcastTitle -->

    <owl:Class rdf:about="http://www.semanticweb.org/cassandwich/ontologies/2018/2/podcast-ontology#PodcastTitle">
        <rdfs:comment>The title of the podcast.</rdfs:comment>
    </owl:Class>
    


    <!-- http://www.semanticweb.org/cassandwich/ontologies/2018/2/podcast-ontology#Radiolab -->

    <owl:Class rdf:about="http://www.semanticweb.org/cassandwich/ontologies/2018/2/podcast-ontology#Radiolab">
        <rdfs:subClassOf rdf:resource="http://www.semanticweb.org/cassandwich/ontologies/2018/2/podcast-ontology#PodcastTitle"/>
        <rdfs:subClassOf>
            <owl:Restriction>
                <owl:onProperty rdf:resource="http://www.semanticweb.org/cassandwich/ontologies/2018/2/podcast-ontology#has_number_of_hosts"/>
                <owl:someValuesFrom rdf:resource="http://www.semanticweb.org/cassandwich/ontologies/2018/2/podcast-ontology#Two"/>
            </owl:Restriction>
        </rdfs:subClassOf>
        <rdfs:subClassOf>
            <owl:Restriction>
                <owl:onProperty rdf:resource="http://www.semanticweb.org/cassandwich/ontologies/2018/2/podcast-ontology#is_genre"/>
                <owl:someValuesFrom rdf:resource="http://www.semanticweb.org/cassandwich/ontologies/2018/2/podcast-ontology#NonFiction"/>
            </owl:Restriction>
        </rdfs:subClassOf>
        <rdfs:subClassOf>
            <owl:Restriction>
                <owl:onProperty rdf:resource="http://www.semanticweb.org/cassandwich/ontologies/2018/2/podcast-ontology#is_categorized_as"/>
                <owl:allValuesFrom rdf:resource="http://www.semanticweb.org/cassandwich/ontologies/2018/2/podcast-ontology#NaturalSciences"/>
            </owl:Restriction>
        </rdfs:subClassOf>
        <rdfs:subClassOf>
            <owl:Restriction>
                <owl:onProperty rdf:resource="http://www.semanticweb.org/cassandwich/ontologies/2018/2/podcast-ontology#is_from_country"/>
                <owl:allValuesFrom rdf:resource="http://www.semanticweb.org/cassandwich/ontologies/2018/2/podcast-ontology#UnitedStates"/>
            </owl:Restriction>
        </rdfs:subClassOf>
        <rdfs:comment>Podcast is titled &apos;Radiolab&apos;.

Reference: https://itunes.apple.com/ca/podcast/radiolab/id152249110?mt=2</rdfs:comment>
    </owl:Class>
    


    <!-- http://www.semanticweb.org/cassandwich/ontologies/2018/2/podcast-ontology#RadiolabPresentsMorePerfect -->

    <owl:Class rdf:about="http://www.semanticweb.org/cassandwich/ontologies/2018/2/podcast-ontology#RadiolabPresentsMorePerfect">
        <rdfs:subClassOf rdf:resource="http://www.semanticweb.org/cassandwich/ontologies/2018/2/podcast-ontology#PodcastTitle"/>
        <rdfs:subClassOf>
            <owl:Restriction>
                <owl:onProperty rdf:resource="http://www.semanticweb.org/cassandwich/ontologies/2018/2/podcast-ontology#has_number_of_hosts"/>
                <owl:someValuesFrom rdf:resource="http://www.semanticweb.org/cassandwich/ontologies/2018/2/podcast-ontology#Two"/>
            </owl:Restriction>
        </rdfs:subClassOf>
        <rdfs:subClassOf>
            <owl:Restriction>
                <owl:onProperty rdf:resource="http://www.semanticweb.org/cassandwich/ontologies/2018/2/podcast-ontology#is_categorized_as"/>
                <owl:allValuesFrom rdf:resource="http://www.semanticweb.org/cassandwich/ontologies/2018/2/podcast-ontology#Government&amp;Organisations"/>
            </owl:Restriction>
        </rdfs:subClassOf>
        <rdfs:subClassOf>
            <owl:Restriction>
                <owl:onProperty rdf:resource="http://www.semanticweb.org/cassandwich/ontologies/2018/2/podcast-ontology#is_from_country"/>
                <owl:allValuesFrom rdf:resource="http://www.semanticweb.org/cassandwich/ontologies/2018/2/podcast-ontology#UnitedStates"/>
            </owl:Restriction>
        </rdfs:subClassOf>
        <rdfs:subClassOf>
            <owl:Restriction>
                <owl:onProperty rdf:resource="http://www.semanticweb.org/cassandwich/ontologies/2018/2/podcast-ontology#is_genre"/>
                <owl:allValuesFrom rdf:resource="http://www.semanticweb.org/cassandwich/ontologies/2018/2/podcast-ontology#NonFiction"/>
            </owl:Restriction>
        </rdfs:subClassOf>
        <rdfs:comment>Podcast is titled &apos;Radiolab Presents: More Perfect&apos;.

Reference: https://itunes.apple.com/ca/podcast/radiolab-presents-more-perfect/id1117202653?mt=2</rdfs:comment>
    </owl:Class>
    


    <!-- http://www.semanticweb.org/cassandwich/ontologies/2018/2/podcast-ontology#RedHanded -->

    <owl:Class rdf:about="http://www.semanticweb.org/cassandwich/ontologies/2018/2/podcast-ontology#RedHanded">
        <rdfs:subClassOf rdf:resource="http://www.semanticweb.org/cassandwich/ontologies/2018/2/podcast-ontology#PodcastTitle"/>
        <rdfs:subClassOf>
            <owl:Restriction>
                <owl:onProperty rdf:resource="http://www.semanticweb.org/cassandwich/ontologies/2018/2/podcast-ontology#has_number_of_hosts"/>
                <owl:allValuesFrom rdf:resource="http://www.semanticweb.org/cassandwich/ontologies/2018/2/podcast-ontology#Two"/>
            </owl:Restriction>
        </rdfs:subClassOf>
        <rdfs:subClassOf>
            <owl:Restriction>
                <owl:onProperty rdf:resource="http://www.semanticweb.org/cassandwich/ontologies/2018/2/podcast-ontology#is_categorized_as"/>
                <owl:allValuesFrom rdf:resource="http://www.semanticweb.org/cassandwich/ontologies/2018/2/podcast-ontology#Society&amp;Culture"/>
            </owl:Restriction>
        </rdfs:subClassOf>
        <rdfs:subClassOf>
            <owl:Restriction>
                <owl:onProperty rdf:resource="http://www.semanticweb.org/cassandwich/ontologies/2018/2/podcast-ontology#is_from_country"/>
                <owl:allValuesFrom rdf:resource="http://www.semanticweb.org/cassandwich/ontologies/2018/2/podcast-ontology#England"/>
            </owl:Restriction>
        </rdfs:subClassOf>
        <rdfs:subClassOf>
            <owl:Restriction>
                <owl:onProperty rdf:resource="http://www.semanticweb.org/cassandwich/ontologies/2018/2/podcast-ontology#is_genre"/>
                <owl:allValuesFrom rdf:resource="http://www.semanticweb.org/cassandwich/ontologies/2018/2/podcast-ontology#NonFiction"/>
            </owl:Restriction>
        </rdfs:subClassOf>
        <rdfs:comment>Podcast is titled &apos;Red Handed&apos;.

Reference: https://itunes.apple.com/us/podcast/redhanded/id1250599915?mt=2</rdfs:comment>
    </owl:Class>
    


    <!-- http://www.semanticweb.org/cassandwich/ontologies/2018/2/podcast-ontology#ReplyAll -->

    <owl:Class rdf:about="http://www.semanticweb.org/cassandwich/ontologies/2018/2/podcast-ontology#ReplyAll">
        <rdfs:subClassOf rdf:resource="http://www.semanticweb.org/cassandwich/ontologies/2018/2/podcast-ontology#PodcastTitle"/>
        <rdfs:subClassOf>
            <owl:Restriction>
                <owl:onProperty rdf:resource="http://www.semanticweb.org/cassandwich/ontologies/2018/2/podcast-ontology#has_number_of_hosts"/>
                <owl:someValuesFrom rdf:resource="http://www.semanticweb.org/cassandwich/ontologies/2018/2/podcast-ontology#Two"/>
            </owl:Restriction>
        </rdfs:subClassOf>
        <rdfs:subClassOf>
            <owl:Restriction>
                <owl:onProperty rdf:resource="http://www.semanticweb.org/cassandwich/ontologies/2018/2/podcast-ontology#is_genre"/>
                <owl:someValuesFrom rdf:resource="http://www.semanticweb.org/cassandwich/ontologies/2018/2/podcast-ontology#NonFiction"/>
            </owl:Restriction>
        </rdfs:subClassOf>
        <rdfs:subClassOf>
            <owl:Restriction>
                <owl:onProperty rdf:resource="http://www.semanticweb.org/cassandwich/ontologies/2018/2/podcast-ontology#is_categorized_as"/>
                <owl:allValuesFrom rdf:resource="http://www.semanticweb.org/cassandwich/ontologies/2018/2/podcast-ontology#Technology"/>
            </owl:Restriction>
        </rdfs:subClassOf>
        <rdfs:subClassOf>
            <owl:Restriction>
                <owl:onProperty rdf:resource="http://www.semanticweb.org/cassandwich/ontologies/2018/2/podcast-ontology#is_from_country"/>
                <owl:allValuesFrom rdf:resource="http://www.semanticweb.org/cassandwich/ontologies/2018/2/podcast-ontology#UnitedStates"/>
            </owl:Restriction>
        </rdfs:subClassOf>
        <rdfs:comment>Podcast is titled &apos;Reply All&apos;.

Reference: https://itunes.apple.com/ca/podcast/reply-all/id941907967?mt=2</rdfs:comment>
    </owl:Class>
    


    <!-- http://www.semanticweb.org/cassandwich/ontologies/2018/2/podcast-ontology#SelfHelp -->

    <owl:Class rdf:about="http://www.semanticweb.org/cassandwich/ontologies/2018/2/podcast-ontology#SelfHelp">
        <rdfs:subClassOf rdf:resource="http://www.semanticweb.org/cassandwich/ontologies/2018/2/podcast-ontology#Health"/>
        <rdfs:comment>The subcategory of the Health category defined by iTunes as Self-Help.

Reference: https://itunes.apple.com/ca/genre/podcasts-health-self-help/id1420?mt=2</rdfs:comment>
    </owl:Class>
    


    <!-- http://www.semanticweb.org/cassandwich/ontologies/2018/2/podcast-ontology#Serial -->

    <owl:Class rdf:about="http://www.semanticweb.org/cassandwich/ontologies/2018/2/podcast-ontology#Serial">
        <rdfs:subClassOf rdf:resource="http://www.semanticweb.org/cassandwich/ontologies/2018/2/podcast-ontology#PodcastTitle"/>
        <rdfs:subClassOf>
            <owl:Restriction>
                <owl:onProperty rdf:resource="http://www.semanticweb.org/cassandwich/ontologies/2018/2/podcast-ontology#has_number_of_hosts"/>
                <owl:someValuesFrom rdf:resource="http://www.semanticweb.org/cassandwich/ontologies/2018/2/podcast-ontology#One"/>
            </owl:Restriction>
        </rdfs:subClassOf>
        <rdfs:subClassOf>
            <owl:Restriction>
                <owl:onProperty rdf:resource="http://www.semanticweb.org/cassandwich/ontologies/2018/2/podcast-ontology#is_categorized_as"/>
                <owl:allValuesFrom rdf:resource="http://www.semanticweb.org/cassandwich/ontologies/2018/2/podcast-ontology#Society&amp;Culture"/>
            </owl:Restriction>
        </rdfs:subClassOf>
        <rdfs:subClassOf>
            <owl:Restriction>
                <owl:onProperty rdf:resource="http://www.semanticweb.org/cassandwich/ontologies/2018/2/podcast-ontology#is_from_country"/>
                <owl:allValuesFrom rdf:resource="http://www.semanticweb.org/cassandwich/ontologies/2018/2/podcast-ontology#UnitedStates"/>
            </owl:Restriction>
        </rdfs:subClassOf>
        <rdfs:subClassOf>
            <owl:Restriction>
                <owl:onProperty rdf:resource="http://www.semanticweb.org/cassandwich/ontologies/2018/2/podcast-ontology#is_genre"/>
                <owl:allValuesFrom rdf:resource="http://www.semanticweb.org/cassandwich/ontologies/2018/2/podcast-ontology#NonFiction"/>
            </owl:Restriction>
        </rdfs:subClassOf>
        <rdfs:comment>Podcast is titled &apos;Serial&apos;.

Reference: https://itunes.apple.com/ca/podcast/serial/id917918570?mt=2</rdfs:comment>
    </owl:Class>
    


    <!-- http://www.semanticweb.org/cassandwich/ontologies/2018/2/podcast-ontology#Six -->

    <owl:Class rdf:about="http://www.semanticweb.org/cassandwich/ontologies/2018/2/podcast-ontology#Six">
        <rdfs:subClassOf rdf:resource="http://www.semanticweb.org/cassandwich/ontologies/2018/2/podcast-ontology#NumberOfHosts"/>
        <rdfs:comment>Six individuals as hosts.</rdfs:comment>
    </owl:Class>
    


    <!-- http://www.semanticweb.org/cassandwich/ontologies/2018/2/podcast-ontology#SocialSciences -->

    <owl:Class rdf:about="http://www.semanticweb.org/cassandwich/ontologies/2018/2/podcast-ontology#SocialSciences">
        <rdfs:subClassOf rdf:resource="http://www.semanticweb.org/cassandwich/ontologies/2018/2/podcast-ontology#Science&amp;Medicine"/>
        <rdfs:comment>The subcategory of the Science &amp; Medicine category defined by iTunes as Social Sciences.

Reference: https://itunes.apple.com/ca/genre/podcasts-science-medicine-social-sciences/id1479?mt=2</rdfs:comment>
    </owl:Class>
    


    <!-- http://www.semanticweb.org/cassandwich/ontologies/2018/2/podcast-ontology#SomeoneKnowsSomething -->

    <owl:Class rdf:about="http://www.semanticweb.org/cassandwich/ontologies/2018/2/podcast-ontology#SomeoneKnowsSomething">
        <rdfs:subClassOf rdf:resource="http://www.semanticweb.org/cassandwich/ontologies/2018/2/podcast-ontology#PodcastTitle"/>
        <rdfs:subClassOf>
            <owl:Restriction>
                <owl:onProperty rdf:resource="http://www.semanticweb.org/cassandwich/ontologies/2018/2/podcast-ontology#has_number_of_hosts"/>
                <owl:allValuesFrom rdf:resource="http://www.semanticweb.org/cassandwich/ontologies/2018/2/podcast-ontology#One"/>
            </owl:Restriction>
        </rdfs:subClassOf>
        <rdfs:subClassOf>
            <owl:Restriction>
                <owl:onProperty rdf:resource="http://www.semanticweb.org/cassandwich/ontologies/2018/2/podcast-ontology#is_categorized_as"/>
                <owl:allValuesFrom rdf:resource="http://www.semanticweb.org/cassandwich/ontologies/2018/2/podcast-ontology#News&amp;Politics"/>
            </owl:Restriction>
        </rdfs:subClassOf>
        <rdfs:subClassOf>
            <owl:Restriction>
                <owl:onProperty rdf:resource="http://www.semanticweb.org/cassandwich/ontologies/2018/2/podcast-ontology#is_from_country"/>
                <owl:allValuesFrom rdf:resource="http://www.semanticweb.org/cassandwich/ontologies/2018/2/podcast-ontology#Canada"/>
            </owl:Restriction>
        </rdfs:subClassOf>
        <rdfs:subClassOf>
            <owl:Restriction>
                <owl:onProperty rdf:resource="http://www.semanticweb.org/cassandwich/ontologies/2018/2/podcast-ontology#is_genre"/>
                <owl:allValuesFrom rdf:resource="http://www.semanticweb.org/cassandwich/ontologies/2018/2/podcast-ontology#NonFiction"/>
            </owl:Restriction>
        </rdfs:subClassOf>
        <rdfs:comment>Podcast is titled &apos;Someone Knows Something&apos;.

Reference: https://itunes.apple.com/ca/podcast/someone-knows-something/id1089216339?mt=2</rdfs:comment>
    </owl:Class>
    


    <!-- http://www.semanticweb.org/cassandwich/ontologies/2018/2/podcast-ontology#SongExploder -->

    <owl:Class rdf:about="http://www.semanticweb.org/cassandwich/ontologies/2018/2/podcast-ontology#SongExploder">
        <rdfs:subClassOf rdf:resource="http://www.semanticweb.org/cassandwich/ontologies/2018/2/podcast-ontology#PodcastTitle"/>
        <rdfs:subClassOf>
            <owl:Restriction>
                <owl:onProperty rdf:resource="http://www.semanticweb.org/cassandwich/ontologies/2018/2/podcast-ontology#has_number_of_hosts"/>
                <owl:someValuesFrom rdf:resource="http://www.semanticweb.org/cassandwich/ontologies/2018/2/podcast-ontology#One"/>
            </owl:Restriction>
        </rdfs:subClassOf>
        <rdfs:subClassOf>
            <owl:Restriction>
                <owl:onProperty rdf:resource="http://www.semanticweb.org/cassandwich/ontologies/2018/2/podcast-ontology#is_categorized_as"/>
                <owl:allValuesFrom rdf:resource="http://www.semanticweb.org/cassandwich/ontologies/2018/2/podcast-ontology#Music"/>
            </owl:Restriction>
        </rdfs:subClassOf>
        <rdfs:subClassOf>
            <owl:Restriction>
                <owl:onProperty rdf:resource="http://www.semanticweb.org/cassandwich/ontologies/2018/2/podcast-ontology#is_from_country"/>
                <owl:allValuesFrom rdf:resource="http://www.semanticweb.org/cassandwich/ontologies/2018/2/podcast-ontology#UnitedStates"/>
            </owl:Restriction>
        </rdfs:subClassOf>
        <rdfs:subClassOf>
            <owl:Restriction>
                <owl:onProperty rdf:resource="http://www.semanticweb.org/cassandwich/ontologies/2018/2/podcast-ontology#is_genre"/>
                <owl:allValuesFrom rdf:resource="http://www.semanticweb.org/cassandwich/ontologies/2018/2/podcast-ontology#NonFiction"/>
            </owl:Restriction>
        </rdfs:subClassOf>
        <rdfs:comment>Podcast is titled &apos;Song Exploder&apos;.

Reference: https://itunes.apple.com/ca/podcast/song-exploder/id788236947?mt=2</rdfs:comment>
    </owl:Class>
    


    <!-- http://www.semanticweb.org/cassandwich/ontologies/2018/2/podcast-ontology#Technology -->

    <owl:Class rdf:about="http://www.semanticweb.org/cassandwich/ontologies/2018/2/podcast-ontology#Technology">
        <rdfs:subClassOf rdf:resource="http://www.semanticweb.org/cassandwich/ontologies/2018/2/podcast-ontology#PodcastCategory"/>
        <rdfs:comment>The category defined by iTunes as Technology.

Reference: https://itunes.apple.com/ca/genre/podcasts-technology/id1318?mt=2</rdfs:comment>
    </owl:Class>
    


    <!-- http://www.semanticweb.org/cassandwich/ontologies/2018/2/podcast-ontology#TheLongestShortestTime -->

    <owl:Class rdf:about="http://www.semanticweb.org/cassandwich/ontologies/2018/2/podcast-ontology#TheLongestShortestTime">
        <rdfs:subClassOf rdf:resource="http://www.semanticweb.org/cassandwich/ontologies/2018/2/podcast-ontology#PodcastTitle"/>
        <rdfs:subClassOf>
            <owl:Restriction>
                <owl:onProperty rdf:resource="http://www.semanticweb.org/cassandwich/ontologies/2018/2/podcast-ontology#has_number_of_hosts"/>
                <owl:someValuesFrom rdf:resource="http://www.semanticweb.org/cassandwich/ontologies/2018/2/podcast-ontology#One"/>
            </owl:Restriction>
        </rdfs:subClassOf>
        <rdfs:subClassOf>
            <owl:Restriction>
                <owl:onProperty rdf:resource="http://www.semanticweb.org/cassandwich/ontologies/2018/2/podcast-ontology#is_genre"/>
                <owl:someValuesFrom rdf:resource="http://www.semanticweb.org/cassandwich/ontologies/2018/2/podcast-ontology#NonFiction"/>
            </owl:Restriction>
        </rdfs:subClassOf>
        <rdfs:subClassOf>
            <owl:Restriction>
                <owl:onProperty rdf:resource="http://www.semanticweb.org/cassandwich/ontologies/2018/2/podcast-ontology#is_categorized_as"/>
                <owl:allValuesFrom rdf:resource="http://www.semanticweb.org/cassandwich/ontologies/2018/2/podcast-ontology#Kids&amp;Family"/>
            </owl:Restriction>
        </rdfs:subClassOf>
        <rdfs:subClassOf>
            <owl:Restriction>
                <owl:onProperty rdf:resource="http://www.semanticweb.org/cassandwich/ontologies/2018/2/podcast-ontology#is_from_country"/>
                <owl:allValuesFrom rdf:resource="http://www.semanticweb.org/cassandwich/ontologies/2018/2/podcast-ontology#UnitedStates"/>
            </owl:Restriction>
        </rdfs:subClassOf>
        <rdfs:comment>Podcast is titled &apos;The Longest Shortest Time&apos;.

Reference: https://itunes.apple.com/ca/podcast/the-longest-shortest-time/id412457621?mt=2</rdfs:comment>
    </owl:Class>
    


    <!-- http://www.semanticweb.org/cassandwich/ontologies/2018/2/podcast-ontology#TheMinimalists -->

    <owl:Class rdf:about="http://www.semanticweb.org/cassandwich/ontologies/2018/2/podcast-ontology#TheMinimalists">
        <rdfs:subClassOf rdf:resource="http://www.semanticweb.org/cassandwich/ontologies/2018/2/podcast-ontology#PodcastTitle"/>
        <rdfs:subClassOf>
            <owl:Restriction>
                <owl:onProperty rdf:resource="http://www.semanticweb.org/cassandwich/ontologies/2018/2/podcast-ontology#has_number_of_hosts"/>
                <owl:allValuesFrom rdf:resource="http://www.semanticweb.org/cassandwich/ontologies/2018/2/podcast-ontology#Two"/>
            </owl:Restriction>
        </rdfs:subClassOf>
        <rdfs:subClassOf>
            <owl:Restriction>
                <owl:onProperty rdf:resource="http://www.semanticweb.org/cassandwich/ontologies/2018/2/podcast-ontology#is_categorized_as"/>
                <owl:allValuesFrom rdf:resource="http://www.semanticweb.org/cassandwich/ontologies/2018/2/podcast-ontology#SelfHelp"/>
            </owl:Restriction>
        </rdfs:subClassOf>
        <rdfs:subClassOf>
            <owl:Restriction>
                <owl:onProperty rdf:resource="http://www.semanticweb.org/cassandwich/ontologies/2018/2/podcast-ontology#is_from_country"/>
                <owl:allValuesFrom rdf:resource="http://www.semanticweb.org/cassandwich/ontologies/2018/2/podcast-ontology#UnitedStates"/>
            </owl:Restriction>
        </rdfs:subClassOf>
        <rdfs:subClassOf>
            <owl:Restriction>
                <owl:onProperty rdf:resource="http://www.semanticweb.org/cassandwich/ontologies/2018/2/podcast-ontology#is_genre"/>
                <owl:allValuesFrom rdf:resource="http://www.semanticweb.org/cassandwich/ontologies/2018/2/podcast-ontology#NonFiction"/>
            </owl:Restriction>
        </rdfs:subClassOf>
        <rdfs:comment>Podcast is titled &apos;The Minimalists&apos;.

Reference: https://itunes.apple.com/ca/podcast/the-minimalists-podcast/id1069757084?mt=2</rdfs:comment>
    </owl:Class>
    


    <!-- http://www.semanticweb.org/cassandwich/ontologies/2018/2/podcast-ontology#ThisAmericanLife -->

    <owl:Class rdf:about="http://www.semanticweb.org/cassandwich/ontologies/2018/2/podcast-ontology#ThisAmericanLife">
        <rdfs:subClassOf rdf:resource="http://www.semanticweb.org/cassandwich/ontologies/2018/2/podcast-ontology#PodcastTitle"/>
        <rdfs:subClassOf>
            <owl:Restriction>
                <owl:onProperty rdf:resource="http://www.semanticweb.org/cassandwich/ontologies/2018/2/podcast-ontology#has_number_of_hosts"/>
                <owl:someValuesFrom rdf:resource="http://www.semanticweb.org/cassandwich/ontologies/2018/2/podcast-ontology#One"/>
            </owl:Restriction>
        </rdfs:subClassOf>
        <rdfs:subClassOf>
            <owl:Restriction>
                <owl:onProperty rdf:resource="http://www.semanticweb.org/cassandwich/ontologies/2018/2/podcast-ontology#is_genre"/>
                <owl:someValuesFrom rdf:resource="http://www.semanticweb.org/cassandwich/ontologies/2018/2/podcast-ontology#NonFiction"/>
            </owl:Restriction>
        </rdfs:subClassOf>
        <rdfs:subClassOf>
            <owl:Restriction>
                <owl:onProperty rdf:resource="http://www.semanticweb.org/cassandwich/ontologies/2018/2/podcast-ontology#is_categorized_as"/>
                <owl:allValuesFrom rdf:resource="http://www.semanticweb.org/cassandwich/ontologies/2018/2/podcast-ontology#PersonalJournals"/>
            </owl:Restriction>
        </rdfs:subClassOf>
        <rdfs:subClassOf>
            <owl:Restriction>
                <owl:onProperty rdf:resource="http://www.semanticweb.org/cassandwich/ontologies/2018/2/podcast-ontology#is_from_country"/>
                <owl:allValuesFrom rdf:resource="http://www.semanticweb.org/cassandwich/ontologies/2018/2/podcast-ontology#UnitedStates"/>
            </owl:Restriction>
        </rdfs:subClassOf>
        <rdfs:comment>Podcast is titled &apos;This American Life&apos;.

Reference: https://itunes.apple.com/ca/podcast/this-american-life/id201671138?mt=2</rdfs:comment>
    </owl:Class>
    


    <!-- http://www.semanticweb.org/cassandwich/ontologies/2018/2/podcast-ontology#Three -->

    <owl:Class rdf:about="http://www.semanticweb.org/cassandwich/ontologies/2018/2/podcast-ontology#Three">
        <rdfs:subClassOf rdf:resource="http://www.semanticweb.org/cassandwich/ontologies/2018/2/podcast-ontology#NumberOfHosts"/>
        <rdfs:comment>Three individuals as hosts.</rdfs:comment>
    </owl:Class>
    


    <!-- http://www.semanticweb.org/cassandwich/ontologies/2018/2/podcast-ontology#Two -->

    <owl:Class rdf:about="http://www.semanticweb.org/cassandwich/ontologies/2018/2/podcast-ontology#Two">
        <rdfs:subClassOf rdf:resource="http://www.semanticweb.org/cassandwich/ontologies/2018/2/podcast-ontology#NumberOfHosts"/>
        <rdfs:comment>Two individuals as hosts.</rdfs:comment>
    </owl:Class>
    


    <!-- http://www.semanticweb.org/cassandwich/ontologies/2018/2/podcast-ontology#UnitedStates -->

    <owl:Class rdf:about="http://www.semanticweb.org/cassandwich/ontologies/2018/2/podcast-ontology#UnitedStates">
        <rdfs:subClassOf rdf:resource="http://www.semanticweb.org/cassandwich/ontologies/2018/2/podcast-ontology#PodcastCountryOfOrigin"/>
        <rdfs:comment>Country of origin is the United States.</rdfs:comment>
    </owl:Class>
    


    <!-- http://www.semanticweb.org/cassandwich/ontologies/2018/2/podcast-ontology#WaitWaitDontTellMe -->

    <owl:Class rdf:about="http://www.semanticweb.org/cassandwich/ontologies/2018/2/podcast-ontology#WaitWaitDontTellMe">
        <rdfs:subClassOf rdf:resource="http://www.semanticweb.org/cassandwich/ontologies/2018/2/podcast-ontology#PodcastTitle"/>
        <rdfs:subClassOf>
            <owl:Restriction>
                <owl:onProperty rdf:resource="http://www.semanticweb.org/cassandwich/ontologies/2018/2/podcast-ontology#has_number_of_hosts"/>
                <owl:someValuesFrom rdf:resource="http://www.semanticweb.org/cassandwich/ontologies/2018/2/podcast-ontology#Five"/>
            </owl:Restriction>
        </rdfs:subClassOf>
        <rdfs:subClassOf>
            <owl:Restriction>
                <owl:onProperty rdf:resource="http://www.semanticweb.org/cassandwich/ontologies/2018/2/podcast-ontology#is_categorized_as"/>
                <owl:allValuesFrom rdf:resource="http://www.semanticweb.org/cassandwich/ontologies/2018/2/podcast-ontology#Comedy"/>
            </owl:Restriction>
        </rdfs:subClassOf>
        <rdfs:subClassOf>
            <owl:Restriction>
                <owl:onProperty rdf:resource="http://www.semanticweb.org/cassandwich/ontologies/2018/2/podcast-ontology#is_from_country"/>
                <owl:allValuesFrom rdf:resource="http://www.semanticweb.org/cassandwich/ontologies/2018/2/podcast-ontology#UnitedStates"/>
            </owl:Restriction>
        </rdfs:subClassOf>
        <rdfs:subClassOf>
            <owl:Restriction>
                <owl:onProperty rdf:resource="http://www.semanticweb.org/cassandwich/ontologies/2018/2/podcast-ontology#is_genre"/>
                <owl:allValuesFrom rdf:resource="http://www.semanticweb.org/cassandwich/ontologies/2018/2/podcast-ontology#NonFiction"/>
            </owl:Restriction>
        </rdfs:subClassOf>
        <rdfs:comment>Podcast is titled &apos;Wait Wait...Don&apos;t Tell Me!&apos;.

Reference: https://itunes.apple.com/ca/podcast/wait-wait-dont-tell-me/id121493804?mt=2</rdfs:comment>
    </owl:Class>
    


    <!-- http://www.semanticweb.org/cassandwich/ontologies/2018/2/podcast-ontology#WelcomeToNightvale -->

    <owl:Class rdf:about="http://www.semanticweb.org/cassandwich/ontologies/2018/2/podcast-ontology#WelcomeToNightvale">
        <rdfs:subClassOf rdf:resource="http://www.semanticweb.org/cassandwich/ontologies/2018/2/podcast-ontology#PodcastTitle"/>
        <rdfs:subClassOf>
            <owl:Restriction>
                <owl:onProperty rdf:resource="http://www.semanticweb.org/cassandwich/ontologies/2018/2/podcast-ontology#has_number_of_hosts"/>
                <owl:someValuesFrom rdf:resource="http://www.semanticweb.org/cassandwich/ontologies/2018/2/podcast-ontology#One"/>
            </owl:Restriction>
        </rdfs:subClassOf>
        <rdfs:subClassOf>
            <owl:Restriction>
                <owl:onProperty rdf:resource="http://www.semanticweb.org/cassandwich/ontologies/2018/2/podcast-ontology#is_categorized_as"/>
                <owl:allValuesFrom rdf:resource="http://www.semanticweb.org/cassandwich/ontologies/2018/2/podcast-ontology#Comedy"/>
            </owl:Restriction>
        </rdfs:subClassOf>
        <rdfs:subClassOf>
            <owl:Restriction>
                <owl:onProperty rdf:resource="http://www.semanticweb.org/cassandwich/ontologies/2018/2/podcast-ontology#is_from_country"/>
                <owl:allValuesFrom rdf:resource="http://www.semanticweb.org/cassandwich/ontologies/2018/2/podcast-ontology#UnitedStates"/>
            </owl:Restriction>
        </rdfs:subClassOf>
        <rdfs:subClassOf>
            <owl:Restriction>
                <owl:onProperty rdf:resource="http://www.semanticweb.org/cassandwich/ontologies/2018/2/podcast-ontology#is_genre"/>
                <owl:allValuesFrom rdf:resource="http://www.semanticweb.org/cassandwich/ontologies/2018/2/podcast-ontology#Fiction"/>
            </owl:Restriction>
        </rdfs:subClassOf>
        <rdfs:comment>Podcast is titled &apos;Welcome to Nightvale&apos;.

Reference: https://itunes.apple.com/ca/podcast/welcome-to-night-vale/id536258179?mt=2</rdfs:comment>
    </owl:Class>
    


    <!-- http://www.semanticweb.org/cassandwich/ontologies/2018/2/podcast-ontology#YouMustRememberThis -->

    <owl:Class rdf:about="http://www.semanticweb.org/cassandwich/ontologies/2018/2/podcast-ontology#YouMustRememberThis">
        <rdfs:subClassOf rdf:resource="http://www.semanticweb.org/cassandwich/ontologies/2018/2/podcast-ontology#PodcastTitle"/>
        <rdfs:subClassOf>
            <owl:Restriction>
                <owl:onProperty rdf:resource="http://www.semanticweb.org/cassandwich/ontologies/2018/2/podcast-ontology#has_number_of_hosts"/>
                <owl:someValuesFrom rdf:resource="http://www.semanticweb.org/cassandwich/ontologies/2018/2/podcast-ontology#One"/>
            </owl:Restriction>
        </rdfs:subClassOf>
        <rdfs:subClassOf>
            <owl:Restriction>
                <owl:onProperty rdf:resource="http://www.semanticweb.org/cassandwich/ontologies/2018/2/podcast-ontology#is_genre"/>
                <owl:someValuesFrom rdf:resource="http://www.semanticweb.org/cassandwich/ontologies/2018/2/podcast-ontology#NonFiction"/>
            </owl:Restriction>
        </rdfs:subClassOf>
        <rdfs:subClassOf>
            <owl:Restriction>
                <owl:onProperty rdf:resource="http://www.semanticweb.org/cassandwich/ontologies/2018/2/podcast-ontology#is_categorized_as"/>
                <owl:allValuesFrom rdf:resource="http://www.semanticweb.org/cassandwich/ontologies/2018/2/podcast-ontology#TV&amp;Movies"/>
            </owl:Restriction>
        </rdfs:subClassOf>
        <rdfs:subClassOf>
            <owl:Restriction>
                <owl:onProperty rdf:resource="http://www.semanticweb.org/cassandwich/ontologies/2018/2/podcast-ontology#is_from_country"/>
                <owl:allValuesFrom rdf:resource="http://www.semanticweb.org/cassandwich/ontologies/2018/2/podcast-ontology#UnitedStates"/>
            </owl:Restriction>
        </rdfs:subClassOf>
        <rdfs:comment>Podcast is titled &apos;You Must Remember This&apos;.

Reference: https://itunes.apple.com/ca/podcast/you-must-remember-this/id858124601?mt=2</rdfs:comment>
    </owl:Class>
    


    <!-- http://www.semanticweb.org/cassandwich/ontologies/2018/2/podcast-ontology#Zealot -->

    <owl:Class rdf:about="http://www.semanticweb.org/cassandwich/ontologies/2018/2/podcast-ontology#Zealot">
        <rdfs:subClassOf rdf:resource="http://www.semanticweb.org/cassandwich/ontologies/2018/2/podcast-ontology#PodcastTitle"/>
        <rdfs:subClassOf>
            <owl:Restriction>
                <owl:onProperty rdf:resource="http://www.semanticweb.org/cassandwich/ontologies/2018/2/podcast-ontology#is_categorized_as"/>
                <owl:allValuesFrom rdf:resource="http://www.semanticweb.org/cassandwich/ontologies/2018/2/podcast-ontology#Comedy"/>
            </owl:Restriction>
        </rdfs:subClassOf>
        <rdfs:subClassOf>
            <owl:Restriction>
                <owl:onProperty rdf:resource="http://www.semanticweb.org/cassandwich/ontologies/2018/2/podcast-ontology#is_from_country"/>
                <owl:allValuesFrom rdf:resource="http://www.semanticweb.org/cassandwich/ontologies/2018/2/podcast-ontology#Australia"/>
            </owl:Restriction>
        </rdfs:subClassOf>
        <rdfs:subClassOf>
            <owl:Restriction>
                <owl:onProperty rdf:resource="http://www.semanticweb.org/cassandwich/ontologies/2018/2/podcast-ontology#is_genre"/>
                <owl:allValuesFrom rdf:resource="http://www.semanticweb.org/cassandwich/ontologies/2018/2/podcast-ontology#NonFiction"/>
            </owl:Restriction>
        </rdfs:subClassOf>
        <rdfs:subClassOf>
            <owl:Restriction>
                <owl:onProperty rdf:resource="http://www.semanticweb.org/cassandwich/ontologies/2018/2/podcast-ontology#has_number_of_hosts"/>
                <owl:minQualifiedCardinality rdf:datatype="http://www.w3.org/2001/XMLSchema#nonNegativeInteger">1</owl:minQualifiedCardinality>
                <owl:onClass rdf:resource="http://www.semanticweb.org/cassandwich/ontologies/2018/2/podcast-ontology#One"/>
            </owl:Restriction>
        </rdfs:subClassOf>
        <rdfs:comment>Podcast is titled &apos;Zealot&apos;.

Reference: https://itunes.apple.com/ca/podcast/zealot/id1245635983?mt=2</rdfs:comment>
    </owl:Class>
    


    <!-- http://www.semanticweb.org/cassandwich/ontologies/2018/2/podcast-ontology#1995 -->

    <owl:Class rdf:about="http://www.semanticweb.org/cassandwich/ontologies/2018/2/podcast-ontology#1995">
        <rdfs:subClassOf rdf:resource="http://www.semanticweb.org/cassandwich/ontologies/2018/2/podcast-ontology#PodcastTitle"/>
        <rdfs:subClassOf>
            <owl:Restriction>
                <owl:onProperty rdf:resource="http://www.semanticweb.org/cassandwich/ontologies/2018/2/podcast-ontology#has_number_of_hosts"/>
                <owl:someValuesFrom rdf:resource="http://www.semanticweb.org/cassandwich/ontologies/2018/2/podcast-ontology#One"/>
            </owl:Restriction>
        </rdfs:subClassOf>
        <rdfs:subClassOf>
            <owl:Restriction>
                <owl:onProperty rdf:resource="http://www.semanticweb.org/cassandwich/ontologies/2018/2/podcast-ontology#is_genre"/>
                <owl:someValuesFrom rdf:resource="http://www.semanticweb.org/cassandwich/ontologies/2018/2/podcast-ontology#NonFiction"/>
            </owl:Restriction>
        </rdfs:subClassOf>
        <rdfs:subClassOf>
            <owl:Restriction>
                <owl:onProperty rdf:resource="http://www.semanticweb.org/cassandwich/ontologies/2018/2/podcast-ontology#is_categorized_as"/>
                <owl:allValuesFrom rdf:resource="http://www.semanticweb.org/cassandwich/ontologies/2018/2/podcast-ontology#News&amp;Politics"/>
            </owl:Restriction>
        </rdfs:subClassOf>
        <rdfs:subClassOf>
            <owl:Restriction>
                <owl:onProperty rdf:resource="http://www.semanticweb.org/cassandwich/ontologies/2018/2/podcast-ontology#is_from_country"/>
                <owl:allValuesFrom rdf:resource="http://www.semanticweb.org/cassandwich/ontologies/2018/2/podcast-ontology#Canada"/>
            </owl:Restriction>
        </rdfs:subClassOf>
        <rdfs:comment>Podcast is titled &apos;1995&apos;.

Reference: https://itunes.apple.com/ca/podcast/1995/id1201927184?mt=2</rdfs:comment>
    </owl:Class>
    


    <!-- http://www.semanticweb.org/cassandwich/ontologies/2018/2/podcast-ontology#2DopeQueens -->

    <owl:Class rdf:about="http://www.semanticweb.org/cassandwich/ontologies/2018/2/podcast-ontology#2DopeQueens">
        <rdfs:subClassOf rdf:resource="http://www.semanticweb.org/cassandwich/ontologies/2018/2/podcast-ontology#PodcastTitle"/>
        <rdfs:subClassOf>
            <owl:Restriction>
                <owl:onProperty rdf:resource="http://www.semanticweb.org/cassandwich/ontologies/2018/2/podcast-ontology#has_number_of_hosts"/>
                <owl:someValuesFrom rdf:resource="http://www.semanticweb.org/cassandwich/ontologies/2018/2/podcast-ontology#Two"/>
            </owl:Restriction>
        </rdfs:subClassOf>
        <rdfs:subClassOf>
            <owl:Restriction>
                <owl:onProperty rdf:resource="http://www.semanticweb.org/cassandwich/ontologies/2018/2/podcast-ontology#is_genre"/>
                <owl:someValuesFrom rdf:resource="http://www.semanticweb.org/cassandwich/ontologies/2018/2/podcast-ontology#NonFiction"/>
            </owl:Restriction>
        </rdfs:subClassOf>
        <rdfs:subClassOf>
            <owl:Restriction>
                <owl:onProperty rdf:resource="http://www.semanticweb.org/cassandwich/ontologies/2018/2/podcast-ontology#is_categorized_as"/>
                <owl:allValuesFrom rdf:resource="http://www.semanticweb.org/cassandwich/ontologies/2018/2/podcast-ontology#Comedy"/>
            </owl:Restriction>
        </rdfs:subClassOf>
        <rdfs:subClassOf>
            <owl:Restriction>
                <owl:onProperty rdf:resource="http://www.semanticweb.org/cassandwich/ontologies/2018/2/podcast-ontology#is_from_country"/>
                <owl:allValuesFrom rdf:resource="http://www.semanticweb.org/cassandwich/ontologies/2018/2/podcast-ontology#UnitedStates"/>
            </owl:Restriction>
        </rdfs:subClassOf>
        <rdfs:comment>Podcast is titled &apos;2 Dope Queens&apos;.

Reference: https://itunes.apple.com/ca/podcast/2-dope-queens/id1097193327?mt=2</rdfs:comment>
    </owl:Class>
    


    <!-- http://www.semanticweb.org/cassandwich/ontologies/2018/2/podcast-ontology#74Seconds -->

    <owl:Class rdf:about="http://www.semanticweb.org/cassandwich/ontologies/2018/2/podcast-ontology#74Seconds">
        <rdfs:subClassOf rdf:resource="http://www.semanticweb.org/cassandwich/ontologies/2018/2/podcast-ontology#PodcastTitle"/>
        <rdfs:subClassOf>
            <owl:Restriction>
                <owl:onProperty rdf:resource="http://www.semanticweb.org/cassandwich/ontologies/2018/2/podcast-ontology#has_number_of_hosts"/>
                <owl:someValuesFrom rdf:resource="http://www.semanticweb.org/cassandwich/ontologies/2018/2/podcast-ontology#One"/>
            </owl:Restriction>
        </rdfs:subClassOf>
        <rdfs:subClassOf>
            <owl:Restriction>
                <owl:onProperty rdf:resource="http://www.semanticweb.org/cassandwich/ontologies/2018/2/podcast-ontology#is_categorized_as"/>
                <owl:allValuesFrom rdf:resource="http://www.semanticweb.org/cassandwich/ontologies/2018/2/podcast-ontology#News&amp;Politics"/>
            </owl:Restriction>
        </rdfs:subClassOf>
        <rdfs:subClassOf>
            <owl:Restriction>
                <owl:onProperty rdf:resource="http://www.semanticweb.org/cassandwich/ontologies/2018/2/podcast-ontology#is_from_country"/>
                <owl:allValuesFrom rdf:resource="http://www.semanticweb.org/cassandwich/ontologies/2018/2/podcast-ontology#UnitedStates"/>
            </owl:Restriction>
        </rdfs:subClassOf>
        <rdfs:subClassOf>
            <owl:Restriction>
                <owl:onProperty rdf:resource="http://www.semanticweb.org/cassandwich/ontologies/2018/2/podcast-ontology#is_genre"/>
                <owl:allValuesFrom rdf:resource="http://www.semanticweb.org/cassandwich/ontologies/2018/2/podcast-ontology#NonFiction"/>
            </owl:Restriction>
        </rdfs:subClassOf>
        <rdfs:comment>Podcast is titled &apos;74 Seconds&apos;.

References: https://itunes.apple.com/gb/podcast/74-seconds/id1237619606?mt=2</rdfs:comment>
    </owl:Class>
    


    <!-- http://www.semanticweb.org/cassandwich/ontologies/2018/2/podcast-ontology#99PercentInvisible -->

    <owl:Class rdf:about="http://www.semanticweb.org/cassandwich/ontologies/2018/2/podcast-ontology#99PercentInvisible">
        <rdfs:subClassOf rdf:resource="http://www.semanticweb.org/cassandwich/ontologies/2018/2/podcast-ontology#PodcastTitle"/>
        <rdfs:subClassOf>
            <owl:Restriction>
                <owl:onProperty rdf:resource="http://www.semanticweb.org/cassandwich/ontologies/2018/2/podcast-ontology#has_number_of_hosts"/>
                <owl:someValuesFrom rdf:resource="http://www.semanticweb.org/cassandwich/ontologies/2018/2/podcast-ontology#One"/>
            </owl:Restriction>
        </rdfs:subClassOf>
        <rdfs:subClassOf>
            <owl:Restriction>
                <owl:onProperty rdf:resource="http://www.semanticweb.org/cassandwich/ontologies/2018/2/podcast-ontology#is_categorized_as"/>
                <owl:allValuesFrom rdf:resource="http://www.semanticweb.org/cassandwich/ontologies/2018/2/podcast-ontology#Design"/>
            </owl:Restriction>
        </rdfs:subClassOf>
        <rdfs:subClassOf>
            <owl:Restriction>
                <owl:onProperty rdf:resource="http://www.semanticweb.org/cassandwich/ontologies/2018/2/podcast-ontology#is_from_country"/>
                <owl:allValuesFrom rdf:resource="http://www.semanticweb.org/cassandwich/ontologies/2018/2/podcast-ontology#UnitedStates"/>
            </owl:Restriction>
        </rdfs:subClassOf>
        <rdfs:subClassOf>
            <owl:Restriction>
                <owl:onProperty rdf:resource="http://www.semanticweb.org/cassandwich/ontologies/2018/2/podcast-ontology#is_genre"/>
                <owl:allValuesFrom rdf:resource="http://www.semanticweb.org/cassandwich/ontologies/2018/2/podcast-ontology#NonFiction"/>
            </owl:Restriction>
        </rdfs:subClassOf>
        <rdfs:comment>Podcast is titled &apos;99% Invisible&apos;.

Reference: https://itunes.apple.com/ca/podcast/99-invisible/id394775318?mt=2</rdfs:comment>
    </owl:Class>
    


    <!-- http://www.semanticweb.org/cassandwich/ontologies/2018/2/podcast-ontology#Games&amp;Hobbies -->

    <owl:Class rdf:about="http://www.semanticweb.org/cassandwich/ontologies/2018/2/podcast-ontology#Games&amp;Hobbies">
        <rdfs:subClassOf rdf:resource="http://www.semanticweb.org/cassandwich/ontologies/2018/2/podcast-ontology#PodcastCategory"/>
        <rdfs:comment>The category defined by iTunes as Games &amp; Hobbies.

Reference: https://itunes.apple.com/ca/genre/podcasts-games-hobbies/id1323?mt=2</rdfs:comment>
    </owl:Class>
    


    <!-- http://www.semanticweb.org/cassandwich/ontologies/2018/2/podcast-ontology#Government&amp;Organisations -->

    <owl:Class rdf:about="http://www.semanticweb.org/cassandwich/ontologies/2018/2/podcast-ontology#Government&amp;Organisations">
        <rdfs:subClassOf rdf:resource="http://www.semanticweb.org/cassandwich/ontologies/2018/2/podcast-ontology#PodcastCategory"/>
        <rdfs:comment>The category defined by iTunes as Government &amp; Organisations.

Reference: https://itunes.apple.com/ca/genre/podcasts-government-organisations/id1325?mt=2</rdfs:comment>
    </owl:Class>
    


    <!-- http://www.semanticweb.org/cassandwich/ontologies/2018/2/podcast-ontology#Kids&amp;Family -->

    <owl:Class rdf:about="http://www.semanticweb.org/cassandwich/ontologies/2018/2/podcast-ontology#Kids&amp;Family">
        <rdfs:subClassOf rdf:resource="http://www.semanticweb.org/cassandwich/ontologies/2018/2/podcast-ontology#PodcastCategory"/>
        <rdfs:comment>The category defined by iTunes as Kids &amp; Family.

Reference: https://itunes.apple.com/ca/genre/podcasts-kids-family/id1305?mt=2</rdfs:comment>
    </owl:Class>
    


    <!-- http://www.semanticweb.org/cassandwich/ontologies/2018/2/podcast-ontology#News&amp;Politics -->

    <owl:Class rdf:about="http://www.semanticweb.org/cassandwich/ontologies/2018/2/podcast-ontology#News&amp;Politics">
        <rdfs:subClassOf rdf:resource="http://www.semanticweb.org/cassandwich/ontologies/2018/2/podcast-ontology#PodcastCategory"/>
        <rdfs:comment>The category defined by iTunes as News &amp; Politics.

Reference: https://itunes.apple.com/ca/genre/podcasts-news-politics/id1311?mt=2</rdfs:comment>
    </owl:Class>
    


    <!-- http://www.semanticweb.org/cassandwich/ontologies/2018/2/podcast-ontology#Religion&amp;Spirituality -->

    <owl:Class rdf:about="http://www.semanticweb.org/cassandwich/ontologies/2018/2/podcast-ontology#Religion&amp;Spirituality">
        <rdfs:subClassOf rdf:resource="http://www.semanticweb.org/cassandwich/ontologies/2018/2/podcast-ontology#PodcastCategory"/>
        <rdfs:comment>The category defined by iTunes as Religion &amp; Spirituality.

Reference: https://itunes.apple.com/ca/genre/podcasts-religion-spirituality/id1314?mt=2</rdfs:comment>
    </owl:Class>
    


    <!-- http://www.semanticweb.org/cassandwich/ontologies/2018/2/podcast-ontology#Science&amp;Medicine -->

    <owl:Class rdf:about="http://www.semanticweb.org/cassandwich/ontologies/2018/2/podcast-ontology#Science&amp;Medicine">
        <rdfs:subClassOf rdf:resource="http://www.semanticweb.org/cassandwich/ontologies/2018/2/podcast-ontology#PodcastCategory"/>
        <rdfs:comment>The category defined by iTunes as Science &amp; Medicine.

Reference: https://itunes.apple.com/ca/genre/podcasts-science-medicine/id1315?mt=2</rdfs:comment>
    </owl:Class>
    


    <!-- http://www.semanticweb.org/cassandwich/ontologies/2018/2/podcast-ontology#Society&amp;Culture -->

    <owl:Class rdf:about="http://www.semanticweb.org/cassandwich/ontologies/2018/2/podcast-ontology#Society&amp;Culture">
        <rdfs:subClassOf rdf:resource="http://www.semanticweb.org/cassandwich/ontologies/2018/2/podcast-ontology#PodcastCategory"/>
        <rdfs:comment>The category defined by iTunes as Society &amp; Culture.

Reference: https://itunes.apple.com/ca/genre/podcasts-society-culture/id1324?mt=2</rdfs:comment>
    </owl:Class>
    


    <!-- http://www.semanticweb.org/cassandwich/ontologies/2018/2/podcast-ontology#Sports&amp;Recreation -->

    <owl:Class rdf:about="http://www.semanticweb.org/cassandwich/ontologies/2018/2/podcast-ontology#Sports&amp;Recreation">
        <rdfs:subClassOf rdf:resource="http://www.semanticweb.org/cassandwich/ontologies/2018/2/podcast-ontology#PodcastCategory"/>
        <rdfs:comment>The category defined by iTunes as Sports &amp; Recreation.

Reference: https://itunes.apple.com/ca/genre/podcasts-sports-recreation/id1316?mt=2</rdfs:comment>
    </owl:Class>
    


    <!-- http://www.semanticweb.org/cassandwich/ontologies/2018/2/podcast-ontology#TV&amp;Movies -->

    <owl:Class rdf:about="http://www.semanticweb.org/cassandwich/ontologies/2018/2/podcast-ontology#TV&amp;Movies">
        <rdfs:subClassOf rdf:resource="http://www.semanticweb.org/cassandwich/ontologies/2018/2/podcast-ontology#PodcastCategory"/>
        <rdfs:comment>The category defined by iTunes as TV &amp; Movies.

Reference: https://itunes.apple.com/ca/genre/podcasts-tv-movies/id1309?mt=2</rdfs:comment>
    </owl:Class>
    


    <!-- http://www.semanticweb.org/cassandwich/ontologies/2018/2/podcast-ontology#TheJay&amp;DanPodcast -->

    <owl:Class rdf:about="http://www.semanticweb.org/cassandwich/ontologies/2018/2/podcast-ontology#TheJay&amp;DanPodcast">
        <rdfs:subClassOf rdf:resource="http://www.semanticweb.org/cassandwich/ontologies/2018/2/podcast-ontology#PodcastTitle"/>
        <rdfs:subClassOf>
            <owl:Restriction>
                <owl:onProperty rdf:resource="http://www.semanticweb.org/cassandwich/ontologies/2018/2/podcast-ontology#has_number_of_hosts"/>
                <owl:someValuesFrom rdf:resource="http://www.semanticweb.org/cassandwich/ontologies/2018/2/podcast-ontology#Two"/>
            </owl:Restriction>
        </rdfs:subClassOf>
        <rdfs:subClassOf>
            <owl:Restriction>
                <owl:onProperty rdf:resource="http://www.semanticweb.org/cassandwich/ontologies/2018/2/podcast-ontology#is_categorized_as"/>
                <owl:allValuesFrom rdf:resource="http://www.semanticweb.org/cassandwich/ontologies/2018/2/podcast-ontology#Sports&amp;Recreation"/>
            </owl:Restriction>
        </rdfs:subClassOf>
        <rdfs:subClassOf>
            <owl:Restriction>
                <owl:onProperty rdf:resource="http://www.semanticweb.org/cassandwich/ontologies/2018/2/podcast-ontology#is_from_country"/>
                <owl:allValuesFrom rdf:resource="http://www.semanticweb.org/cassandwich/ontologies/2018/2/podcast-ontology#Canada"/>
            </owl:Restriction>
        </rdfs:subClassOf>
        <rdfs:subClassOf>
            <owl:Restriction>
                <owl:onProperty rdf:resource="http://www.semanticweb.org/cassandwich/ontologies/2018/2/podcast-ontology#is_genre"/>
                <owl:allValuesFrom rdf:resource="http://www.semanticweb.org/cassandwich/ontologies/2018/2/podcast-ontology#NonFiction"/>
            </owl:Restriction>
        </rdfs:subClassOf>
        <rdfs:comment>Podcast is titled &apos;The Jay &amp; Dan Podcast&apos;.

Reference: https://itunes.apple.com/ca/podcast/the-jay-dan-podcast/id690863774?mt=2</rdfs:comment>
    </owl:Class>
    


    <!-- 
    ///////////////////////////////////////////////////////////////////////////////////////
    //
    // General axioms
    //
    ///////////////////////////////////////////////////////////////////////////////////////
     -->

    <rdf:Description>
        <rdf:type rdf:resource="http://www.w3.org/2002/07/owl#AllDisjointClasses"/>
        <owl:members rdf:parseType="Collection">
            <rdf:Description rdf:about="http://www.semanticweb.org/cassandwich/ontologies/2018/2/podcast-ontology#Arts"/>
            <rdf:Description rdf:about="http://www.semanticweb.org/cassandwich/ontologies/2018/2/podcast-ontology#Business"/>
            <rdf:Description rdf:about="http://www.semanticweb.org/cassandwich/ontologies/2018/2/podcast-ontology#Comedy"/>
            <rdf:Description rdf:about="http://www.semanticweb.org/cassandwich/ontologies/2018/2/podcast-ontology#Education"/>
            <rdf:Description rdf:about="http://www.semanticweb.org/cassandwich/ontologies/2018/2/podcast-ontology#Health"/>
            <rdf:Description rdf:about="http://www.semanticweb.org/cassandwich/ontologies/2018/2/podcast-ontology#Music"/>
            <rdf:Description rdf:about="http://www.semanticweb.org/cassandwich/ontologies/2018/2/podcast-ontology#Technology"/>
            <rdf:Description rdf:about="http://www.semanticweb.org/cassandwich/ontologies/2018/2/podcast-ontology#Games&amp;Hobbies"/>
            <rdf:Description rdf:about="http://www.semanticweb.org/cassandwich/ontologies/2018/2/podcast-ontology#Government&amp;Organisations"/>
            <rdf:Description rdf:about="http://www.semanticweb.org/cassandwich/ontologies/2018/2/podcast-ontology#Kids&amp;Family"/>
            <rdf:Description rdf:about="http://www.semanticweb.org/cassandwich/ontologies/2018/2/podcast-ontology#News&amp;Politics"/>
            <rdf:Description rdf:about="http://www.semanticweb.org/cassandwich/ontologies/2018/2/podcast-ontology#Religion&amp;Spirituality"/>
            <rdf:Description rdf:about="http://www.semanticweb.org/cassandwich/ontologies/2018/2/podcast-ontology#Science&amp;Medicine"/>
            <rdf:Description rdf:about="http://www.semanticweb.org/cassandwich/ontologies/2018/2/podcast-ontology#Society&amp;Culture"/>
            <rdf:Description rdf:about="http://www.semanticweb.org/cassandwich/ontologies/2018/2/podcast-ontology#Sports&amp;Recreation"/>
            <rdf:Description rdf:about="http://www.semanticweb.org/cassandwich/ontologies/2018/2/podcast-ontology#TV&amp;Movies"/>
        </owl:members>
    </rdf:Description>
    <rdf:Description>
        <rdf:type rdf:resource="http://www.w3.org/2002/07/owl#AllDisjointClasses"/>
        <owl:members rdf:parseType="Collection">
            <rdf:Description rdf:about="http://www.semanticweb.org/cassandwich/ontologies/2018/2/podcast-ontology#Australia"/>
            <rdf:Description rdf:about="http://www.semanticweb.org/cassandwich/ontologies/2018/2/podcast-ontology#Canada"/>
            <rdf:Description rdf:about="http://www.semanticweb.org/cassandwich/ontologies/2018/2/podcast-ontology#England"/>
            <rdf:Description rdf:about="http://www.semanticweb.org/cassandwich/ontologies/2018/2/podcast-ontology#NewZealand"/>
            <rdf:Description rdf:about="http://www.semanticweb.org/cassandwich/ontologies/2018/2/podcast-ontology#UnitedStates"/>
        </owl:members>
    </rdf:Description>
    <rdf:Description>
        <rdf:type rdf:resource="http://www.w3.org/2002/07/owl#AllDisjointClasses"/>
        <owl:members rdf:parseType="Collection">
            <rdf:Description rdf:about="http://www.semanticweb.org/cassandwich/ontologies/2018/2/podcast-ontology#Australia"/>
            <rdf:Description rdf:about="http://www.semanticweb.org/cassandwich/ontologies/2018/2/podcast-ontology#Canada"/>
            <rdf:Description rdf:about="http://www.semanticweb.org/cassandwich/ontologies/2018/2/podcast-ontology#England"/>
            <rdf:Description rdf:about="http://www.semanticweb.org/cassandwich/ontologies/2018/2/podcast-ontology#UnitedStates"/>
        </owl:members>
    </rdf:Description>
    <rdf:Description>
        <rdf:type rdf:resource="http://www.w3.org/2002/07/owl#AllDisjointClasses"/>
        <owl:members rdf:parseType="Collection">
            <rdf:Description rdf:about="http://www.semanticweb.org/cassandwich/ontologies/2018/2/podcast-ontology#Five"/>
            <rdf:Description rdf:about="http://www.semanticweb.org/cassandwich/ontologies/2018/2/podcast-ontology#Four"/>
            <rdf:Description rdf:about="http://www.semanticweb.org/cassandwich/ontologies/2018/2/podcast-ontology#One"/>
            <rdf:Description rdf:about="http://www.semanticweb.org/cassandwich/ontologies/2018/2/podcast-ontology#Six"/>
            <rdf:Description rdf:about="http://www.semanticweb.org/cassandwich/ontologies/2018/2/podcast-ontology#Three"/>
            <rdf:Description rdf:about="http://www.semanticweb.org/cassandwich/ontologies/2018/2/podcast-ontology#Two"/>
        </owl:members>
    </rdf:Description>
</rdf:RDF>



<!-- Generated by the OWL API (version 4.2.8.20170104-2310) https://github.com/owlcs/owlapi -->

